Attempt at permutation lemma, but removing an element from a permutation is defined wrong

examples/Yield/Par2.v
@@ -112,9 +112,9 @@ Proof.
   - split. lia. invert. apply H1.
 Qed.
 
-Lemma trans_choiceI_bound E R (t t' : ctree E R) :
+Lemma trans_choiceI_bound E R (t t' : ctree E R) l :
   choiceI_bound 1 t ->
-  trans tau t t' ->
+  trans l t t' ->
   choiceI_bound 1 t'.
 Proof.
   intros Hbound Htrans. revert Hbound.
@@ -128,6 +128,12 @@ Proof.
     assert (t ≅ ChoiceV n k).
     { rewrite ctree_eta. rewrite <- x1. reflexivity. }
     rewrite H1 in Hbound. rewrite H0. step in Hbound. inv Hbound. invert. auto.
+  - assert (t' ≅ k x0).
+    { rewrite ctree_eta. rewrite <- x. rewrite H. rewrite <- ctree_eta. reflexivity. }
+    assert (t ≅ Vis e k).
+    { rewrite ctree_eta. rewrite <- x1. reflexivity. }
+    rewrite H1 in Hbound. rewrite H0. step in Hbound. inv Hbound. invert. auto.
+  - rewrite ctree_eta. rewrite <- x. step. constructor; auto. intros. inv i.
 Qed.
 
 Lemma visible_choiceI_bound E R n (t t' : ctree E R) :
@@ -418,6 +424,13 @@ Section parallel.
     repeat intro. apply H.
   Qed.
 
+  Lemma remove_front_vec_choiceI_bound n n' (v : vec (S n)) :
+    (forall i, choiceI_bound n' (v i)) ->
+    forall i, choiceI_bound n' (remove_front_vec v i).
+  Proof.
+    repeat intro. apply H.
+  Qed.
+
   Equations remove_vec {n : nat} (v : vec (S n)) (i : fin (S n)) : vec n :=
     remove_vec v F1     i'      := remove_front_vec v i';
     remove_vec v (FS i) F1      := v F1;
@@ -435,6 +448,106 @@ Section parallel.
     repeat intro. apply remove_front_vec_vec_relation; auto.
   Qed.
 
+  Lemma remove_vec_choiceI_bound n n' (v : vec (S n)) i' :
+    (forall i, choiceI_bound n' (v i)) ->
+    forall i, choiceI_bound n' (remove_vec v i' i).
+  Proof.
+    intros. depind i'.
+    - apply remove_front_vec_choiceI_bound; auto.
+    - destruct i; cbn; auto.
+      apply IHi'; auto. intros. apply remove_front_vec_choiceI_bound; auto.
+  Qed.
+
+  Lemma remove_vec_remove_vec_front n (v : vec (S (S n))) i i' :
+    remove_vec (remove_front_vec v) i i' = remove_front_vec (remove_vec v (FS i)) i'.
+  Proof.
+    depind i; cbn; auto.
+  Qed.
+
+  (* Lemma of_nat_lt_S n j (Hj : j < S n) (Hj' : j < n) : *)
+  (*   of_nat_lt Hj = FS (of_nat_lt Hj'). *)
+  (* Proof. *)
+  (*   revert n Hj Hj'. *)
+  (*   induction j; intros; auto. *)
+  (*   - cbn. destruct n; auto. inv Hj'. *)
+  (* Qed. *)
+
+  (* before the element removed, the same index works *)
+  Lemma remove_vec_index_before {n} (v : vec (S n)) i j
+        (Hi : i < S n) (Hji : j < i) (Hj : j < S n) (Hj' : j < n) :
+    v (of_nat_lt Hj) = (remove_vec v (of_nat_lt Hi)) (of_nat_lt Hj').
+  Proof.
+    revert n v j Hi Hj Hj' Hji. induction i; intros; auto. inv Hji.
+    destruct n. inv Hj'. destruct j; auto. cbn.
+    erewrite <- IHi; auto. lia.
+  Qed.
+
+  (* after the element removed, we need to subtract one from the index *)
+  Lemma remove_vec_index_after {n} (v : vec (S n)) i j
+        (Hi : i < S n) (Hji : j > i) (Hj : S j < S n) (Hj' : j < n) (* S j to j *) :
+    v (of_nat_lt Hj) = (remove_vec v (of_nat_lt Hi)) (of_nat_lt Hj').
+  Proof.
+    revert n v i Hi Hji Hj Hj'. induction j; intros. inv Hji.
+    destruct i.
+    - destruct n. inv Hj'. cbn. unfold remove_front_vec. erewrite of_nat_ext. reflexivity.
+    - destruct n. inv Hj'. cbn. erewrite <- IHj; eauto. lia.
+  Qed.
+
+  (* at the element removed, we also subtract one. TODO: can we unify this with prev lemma? *)
+  Lemma remove_vec_index_eq {n} (v : vec (S n)) i j
+        (Hi : i < S n) (Hji : j = i) (Hj : S j < S n) (Hj' : j < n) :
+    v (of_nat_lt Hj) = (remove_vec v (of_nat_lt Hi)) (of_nat_lt Hj').
+  Proof.
+    revert n v j Hi Hj Hj' Hji. induction i; intros; auto.
+    - destruct n. inv Hj'. subst. reflexivity.
+    - destruct n. inv Hj'. subst. cbn.
+      erewrite <- IHi; auto.
+  Qed.
+
+  (* Definition remove_vec_index {n} (v : vec (S n)) (i i' : fin (S n)) (H : i <> i') : *)
+  (*   { j : fin n | v i' = (remove_vec v i) j }. *)
+  (*   revert v. depind i; cbn; intros. *)
+  (*   - dependent destruction i'. contradiction. *)
+  (*     exists i'. reflexivity. *)
+  (*   - destruct n; [inv i |]. *)
+  (*     dependent destruction i'; auto. *)
+  (*     + exists F1. reflexivity. *)
+  (*     + assert (i <> i'). { intro. subst. contradiction. } *)
+  (*       edestruct IHi as (j & Hj); eauto. exists (FS j). rewrite <- Hj. reflexivity. *)
+  (* Defined. *)
+
+  (* Lemma remove_vec_index_foo {n} (v : vec (S n)) i j1 j2 Hj1 Hj2 : *)
+  (*   (* TODO: figure out why this doesn't work with ` notation *) *)
+
+  (*   (proj1_sig (remove_vec_index v i (FS j1) Hj1)) <> *)
+  (*     (proj1_sig (remove_vec_index v i (FS j2) Hj2)) -> *)
+  (*   (proj1_sig (remove_vec_index v i j1 Hj1)) <> *)
+  (*     (proj1_sig (remove_vec_index v i j2 Hj2)). *)
+
+  (* Lemma remove_vec_index_injective {n} (v : vec (S n)) i j1 j2 Hj1 Hj2 : *)
+  (*   (* TODO: figure out why this doesn't work with ` notation *) *)
+  (*   j1 <> j2 -> *)
+  (*   (proj1_sig (remove_vec_index v i j1 Hj1)) <> (proj1_sig (remove_vec_index v i j2 Hj2)). *)
+  (* Proof. *)
+  (*   revert v. depind i. *)
+  (*   - intro. intro. revert j2 Hj2 H v. depind j1; [contradiction |]; intros. *)
+  (*     dependent destruction j2; [contradiction |]. destruct n. inv j1. *)
+  (*     apply IHj1. *)
+  (* Qed. *)
+
+  (* Lemma remove_vec_index {n} (v : vec (S n)) i : *)
+  (*   forall i', i <> i' -> exists j, v i' = remove_vec v i j. *)
+  (* Proof. *)
+  (*   revert v. depind i; cbn; intros. *)
+  (*   - dependent destruction i'. contradiction. *)
+  (*     exists i'. reflexivity. *)
+  (*   - destruct n; [inv i |]. *)
+  (*     dependent destruction i'; auto. *)
+  (*     + exists F1. reflexivity. *)
+  (*     + assert (i <> i'). { intro. subst. contradiction. } *)
+  (*       edestruct IHi as (j & Hj); eauto. exists (FS j). rewrite <- Hj. reflexivity. *)
+  (* Qed. *)
+
   Definition remove_vec_helper n n' (v : vec n) (i : fin n) (H : n = S n')
     : vec n'.
     subst. apply remove_vec; eauto.
@@ -444,7 +557,7 @@ Section parallel.
     fun i' => if Fin.eqb i i' then t else v i'.
 
   Lemma remove_front_vec_replace_vec n (v : vec (S n)) i t :
-    remove_front_vec (replace_vec v (Fin.FS i) t) =
+    remove_front_vec (replace_vec v (FS i) t) =
       replace_vec (remove_front_vec v) i t.
   Proof. reflexivity. Qed.
 
@@ -472,6 +585,14 @@ Section parallel.
     unfold replace_vec. repeat intro. destruct (Fin.eqb i i0); auto.
   Qed.
 
+  Lemma replace_vec_choiceI_bound n n' (v : vec n) i' t :
+    (forall i, choiceI_bound n' (v i)) ->
+    choiceI_bound n' t ->
+    forall i, choiceI_bound n' (replace_vec v i' t i).
+  Proof.
+    unfold replace_vec. repeat intro. destruct (Fin.eqb i' i); auto.
+  Qed.
+
   Lemma replace_vec_twice n (v : vec n) i t1 t2 :
     replace_vec (replace_vec v i t1) i t2 = replace_vec v i t2.
   Proof.
@@ -487,13 +608,24 @@ Section parallel.
     reflexivity.
   Qed.
 
-  Lemma replace_vec_same n (v : vec n) i :
-    replace_vec v i (v i) = v.
+  Lemma replace_vec_neq n (v : vec n) i1 i2 t :
+    i1 <> i2 ->
+    (replace_vec v i1 t) i2 = v i2.
   Proof.
-    unfold replace_vec. apply functional_extensionality. intro.
-    destruct (Fin.eqb i x) eqn:?; auto.
-    apply Fin.eqb_eq in Heqb. subst. auto.
+    intros.
+    unfold replace_vec.
+    destruct (Fin.eqb i1 i2) eqn:?.
+    - apply Fin.eqb_eq in Heqb. contradiction.
+    - reflexivity.
   Qed.
+
+  (* Lemma replace_vec_same n (v : vec n) i : *)
+  (*   replace_vec v i (v i) = v. *)
+  (* Proof. *)
+  (*   unfold replace_vec. apply functional_extensionality. intro. *)
+  (*   destruct (Fin.eqb i x) eqn:?; auto. *)
+  (*   apply Fin.eqb_eq in Heqb. subst. auto. *)
+  (* Qed. *)
 
   Equations cons_vec {n : nat} (t : thread) (v : vec n) : vec (S n) :=
     cons_vec t v F1      := t;
@@ -507,6 +639,45 @@ Section parallel.
   Proof.
     unfold cons_vec. repeat intro. depind i; cbn; auto.
   Qed.
+
+  Lemma cons_vec_choiceI_bound n n' (v : vec n) t :
+    (forall i, choiceI_bound n' (v i)) ->
+    choiceI_bound n' t ->
+    forall i, choiceI_bound n' (cons_vec t v i).
+  Proof.
+    unfold cons_vec. repeat intro. depind i; cbn; auto.
+  Qed.
+
+  Lemma remove_vec_cons_1 t1 t2 :
+    (remove_vec (cons_vec t1 (fun _ : fin 1 => t2)) F1) = (fun _ => t2).
+  Proof.
+    apply functional_extensionality. intros i. dependent destruction i; [| inv i].
+    simp remove_vec. unfold remove_front_vec. simp cons_vec. reflexivity.
+  Qed.
+
+  Lemma remove_vec_cons_2 t1 t2 :
+    (remove_vec (cons_vec t1 (fun _ : fin 1 => t2)) (FS F1)) = (fun _ => t1).
+  Proof.
+    apply functional_extensionality. intros i. dependent destruction i; [| inv i].
+    simp remove_vec. simp cons_vec. reflexivity.
+  Qed.
+
+  Lemma replace_vec_cons_1 t1 t2 t :
+    (replace_vec (cons_vec t1 (fun _ : fin 1 => t2)) F1 t) =
+      (cons_vec t (fun _ : fin 1 => t2)).
+  Proof.
+    apply functional_extensionality. intros i. dependent destruction i; reflexivity.
+  Qed.
+
+  Lemma replace_vec_cons_2 t1 t2 t :
+    (replace_vec (cons_vec t1 (fun _ : fin 1 => t2)) (FS F1) t) =
+      (cons_vec t1 (fun _ : fin 1 => t)).
+  Proof.
+    apply functional_extensionality. intros i. dependent destruction i; cbn.
+    - reflexivity.
+    - dependent destruction i; [| inv i]. cbn. simp cons_vec. reflexivity.
+  Qed.
+
 
 
   (* Program Definition append_vec {n : nat} (v : vec n) (t : thread) : vec (S n) := *)
@@ -566,9 +737,10 @@ Section parallel.
         schedule_match _ _ _ _ (VisF (inr1 (inl1 Spawn)) k) :=
           TauV (schedule
                   (S (S n))
+                  (* Note that [cons_vec] puts the new thread on the front of the vector *)
                   (cons_vec (k true) (replace_vec v i (k false)))
                   (* The [i] here means that we don't yield at a spawn *)
-                  (Some (Fin.L_R 1 i))); (* view [i] as a [fin (n + 1)] *)
+                  (Some (FS i))); (* view [i] as a [fin (n + 1)] *)
 
         (* todo *)
         schedule_match _ _ _ _ (VisF (inr1 (inr1 s)) k) :=
@@ -787,7 +959,7 @@ Section parallel.
               t ≅ schedule
                 (S n)
                 (cons_vec (k true) (replace_vec v i (k false)))
-                (Some (Fin.L_R 1 i))).
+                (Some (FS i))).
   Proof.
     unfold trans. intros. cbn in H. red in H. (* destruct n; try inv i. *)
     remember (observe (schedule n v (Some i))).
@@ -972,7 +1144,7 @@ Section parallel.
           (schedule (S (S n))
                     (cons_vec (k true)
                               (replace_vec v i (k false)))
-                    (Some (Fin.L_R 1 i))).
+                    (Some (FS i))).
   Proof.
     intros. cbn in *. red in H |- *. red.
     remember (observe (v i)). remember (observe (Vis _ k)).
@@ -990,7 +1162,7 @@ Section parallel.
       eapply IHvisible_; auto; rewrite replace_vec_eq; eauto.
     - invert.
       rewrite rewrite_schedule at 1. simp schedule_match.
-      rewrite <- Heqc. econstructor. apply Fin.F1. apply equ_schedule.
+      rewrite <- Heqc. econstructor. apply F1. apply equ_schedule.
       apply cons_vec_vec_relation; auto.
       apply replace_vec_vec_relation; repeat intro; auto.
   Qed.
@@ -1044,7 +1216,7 @@ Section parallel.
           destruct H0 as (t' & Ht & Hbound & Hequ).
           pose proof (Hv i) as (Hsb & Hbound1 & Hbound2). step in Hsb. destruct Hsb as [Hf _].
           edestruct Hf as [? ? ?]; eauto.
-          pose proof (trans_choiceI_bound _ _ _ _ Hbound2 H).
+          pose proof (trans_choiceI_bound _ _ _ _ _ Hbound2 H).
           apply trans_thread_schedule_tau in H.
           eexists; eauto. rewrite Hequ. apply CIH.
           apply replace_vec_vec_relation; auto.
@@ -1072,7 +1244,7 @@ Section parallel.
           exists (schedule (S n)
                       (cons_vec (k' true)
                                 (replace_vec v2 i (k' false)))
-                      (Some (Fin.L_R 1 i))).
+                      (Some (FS i))).
           2: { rewrite Hequ. apply CIH. apply cons_vec_vec_relation; auto.
                - apply replace_vec_vec_relation; auto; split; auto. split.
                  + pose proof (visible_choiceI_bound _ _ _ _ _ Hbound1 Hvis).
@@ -1123,4 +1295,2790 @@ Section parallel.
         * rewrite H. reflexivity.
   Qed.
 
+  Lemma of_nat_lt_sig1_neq_1 n1 n2 n (H1 : n1 < n) (H2 : n2 < n) :
+    of_nat_lt H1 <> of_nat_lt H2 ->
+    n1 <> n2.
+  Proof.
+    repeat intro. subst. apply H. apply of_nat_ext.
+  Qed.
+
+  Lemma of_nat_lt_sig1_neq_2 n1 n2 n (H1 : n1 < n) (H2 : n2 < n) :
+    n1 <> n2 ->
+    of_nat_lt H1 <> of_nat_lt H2.
+  Proof.
+    revert n2 n H1 H2. induction n1; intros; auto.
+    - destruct n2; auto. destruct n; [inv H2 |]. intro. inv H0.
+    - destruct n; [inv H2 |]. destruct n2.
+      + intro. inv H0.
+      + cbn. intro. inv H0. invert. eapply (IHn1 n2).
+        * intro. subst. contradiction.
+        * apply x.
+  Qed.
+
+  Lemma of_nat_lt_sig1_neq n1 n2 n (H1 : n1 < n) (H2 : n2 < n) :
+    n1 <> n2 <->
+      of_nat_lt H1 <> of_nat_lt H2.
+  Proof.
+    split. apply of_nat_lt_sig1_neq_2. apply of_nat_lt_sig1_neq_1.
+  Qed.
+
+  (* Definition permutation_from_nat {n} (p q : nat -> nat) *)
+  (*            (Hp : forall i, i < n -> p i < n) *)
+  (*            (Hq : forall i, i < n -> q i < n) *)
+  (*            (Hpq : forall i, i < n -> p (q i) = i) *)
+  (*            (Hqp : forall i, i < n -> q (p i) = i) : *)
+  (*   { x : (fin n -> fin n) * (fin n -> fin n) & *)
+  (*           (forall i, (fst x) ((snd x) i) = i) & *)
+  (*           (forall i, (snd x) ((fst x) i) = i) }. *)
+  (* Proof. *)
+  (*   eexists. Unshelve. *)
+  (*   3: { *)
+  (*     split. *)
+  (*     - intro i. destruct (to_nat i). *)
+  (*       pose proof (Hp x l). *)
+  (*       apply (of_nat_lt H). *)
+  (*     - intro i. destruct (to_nat i). *)
+  (*       pose proof (Hq x l). *)
+  (*       apply (of_nat_lt H). *)
+  (*   } *)
+  (*   - cbn. intros. destruct (to_nat i). *)
+  (*     rewrite to_nat_of_nat. *)
+  (*     erewrite of_nat_ext. *)
+  (*     unfold of_nat_lt. *)
+  (*     (* generalize dependent x. *) *)
+  (*     rewrite (Hpq x l). *)
+  (*     revert (p (q x)). erewrite (Hpq x). *)
+  (* Qed. *)
+
+  (*
+  Definition permutation_to_nat {n} (p q : fin n -> fin n)
+        (Hpq : forall i, p (q i) = i)
+        (Hqp : forall i, q (p i) = i) :
+    { x : (nat -> nat) * (nat -> nat) &
+            (forall i, i < n -> (fst x) i < n) /\ (forall i, i < n -> (snd x) i < n) /\
+            (forall i, i < n -> (fst x) ((snd x) i) = i) /\ (forall i, i < n -> (snd x) ((fst x) i) = i) }.
+  Proof.
+    eexists. Unshelve.
+    2: {
+      split.
+      - clear q Hpq Hqp. intro i'.
+        destruct (Compare_dec.lt_dec i' n).
+        + pose proof (of_nat_lt l) as i.
+          pose proof (p i) as pi.
+          destruct (to_nat pi). apply x.
+        + apply i'.
+      - clear p Hpq Hqp. intro i'.
+        destruct (Compare_dec.lt_dec i' n).
+        + pose proof (of_nat_lt l) as i.
+          pose proof (q i) as qi.
+          destruct (to_nat qi). apply x.
+        + apply i'.
+    }
+    cbn. split; [| split; [| split]].
+    - intros.
+      destruct (Compare_dec.lt_dec i n); try contradiction.
+      destruct (to_nat (q (of_nat_lt l))) eqn:?.
+      destruct (to_nat (p (of_nat_lt l))) eqn:?. auto.
+    - intros.
+      destruct (Compare_dec.lt_dec i n); try contradiction.
+      destruct (to_nat (q (of_nat_lt l))) eqn:?.
+      destruct (to_nat (p (of_nat_lt l))) eqn:?. auto.
+    - intros i Hi.
+      destruct (Compare_dec.lt_dec i n); try contradiction. clear Hi. rename l into Hi.
+      destruct (to_nat (q (of_nat_lt Hi))) as (qi' & Hqi) eqn:?.
+      destruct (Compare_dec.lt_dec qi' n); try contradiction.
+      rewrite (of_nat_ext _ Hqi). clear l.
+      destruct (to_nat (p (of_nat_lt Hqi))) as (pqi' & Hpqi) eqn:?.
+
+      pose proof Heqs as ?. apply (f_equal from_nat_) in H.
+      (* unfold to_nat in Heqs. *)
+      pose proof (Hpq (of_nat_lt Hi)). rewrite <- H in Heqs.
+  Qed. *)
+
+  Definition cons_permutation {n} (p : fin n -> fin n) :
+    {
+      p' : (fin (S n) -> fin (S n)) &
+             p' F1 = F1 /\ forall i, p' (FS i) = FS (p i)
+    }.
+    eexists. Unshelve.
+    2: {
+      intro i.
+      dependent destruction i.
+      - apply F1.
+      - apply (FS (p i)).
+    }
+    split; auto.
+  Defined.
+
+  Lemma cons_permutation_correct {n} (p q : fin n -> fin n)
+        (Hpq : forall i, p (q i) = i)
+        (Hqp : forall i, q (p i) = i) :
+    let p' := projT1 (cons_permutation p) in
+    let q' := projT1 (cons_permutation q) in
+    (forall i, p' (q' i) = i) /\ (forall i, q' (p' i) = i).
+  Proof.
+    destruct (cons_permutation p) as (p' & Hp1 & Hp2).
+    destruct (cons_permutation q) as (q' & Hq1 & Hq2).
+    cbn in *. split.
+    - intro i. dependent destruction i.
+      + rewrite Hq1, Hp1. auto.
+      + rewrite Hq2, Hp2, Hpq. auto.
+    - intro i. dependent destruction i.
+      + rewrite Hp1, Hq1. auto.
+      + rewrite Hp2, Hq2, Hqp. auto.
+  Qed.
+
+  (* Inductive lt {m n} : fin (S m) -> fin (S n) -> Prop := *)
+  (* | lt_base : forall i, lt F1 (FS i) *)
+  (* | lt_ind : forall i j, lt i j -> lt (FS i) (FS j) *)
+  (* . *)
+
+  Variant ordering := LT | EQ | GT.
+
+  Fixpoint order {m n} (p : fin m) (q : fin n) : ordering :=
+    match p, q with
+    | F1, F1 => EQ
+    | F1, _ => LT
+    | _, F1 => GT
+    | FS p', FS q' => order p' q'
+    end.
+
+  Lemma order_reflexive {n} (p : fin n) :
+    order p p = EQ.
+  Proof.
+    depind p; auto.
+  Qed.
+
+  Lemma order_flip {m n} (p : fin m) (q : fin n) :
+    order p q = LT <-> order q p = GT.
+  Proof.
+    split.
+    {
+      revert n q.
+      depind p; dependent destruction q; auto.
+      - intros. inv H.
+      - cbn. eapply IHp.
+    }
+    {
+      revert n q.
+      depind p; dependent destruction q; auto.
+      - intros. inv H.
+      - cbn. eapply IHp.
+    }
+  Qed.
+
+  Lemma order_eq {n} (p q : fin n) :
+    order p q = EQ -> p = q.
+  Proof.
+    depind p; intros; dependent destruction q; inv H; auto.
+    f_equal. auto.
+  Qed.
+
+  Lemma order_e_FS {m n} (p : fin m) (q : fin n) :
+    order p q = EQ -> order (FS p) q = GT.
+  Proof.
+    revert n q.
+    depind p.
+    - intros. dependent destruction q; inv H; auto.
+    - intros. dependent destruction q. inv H. cbn in H. apply IHp; auto.
+  Qed.
+
+  Lemma order_g_FS {m n} (p : fin m) (q : fin n) :
+    order p q = GT -> order (FS p) q = GT.
+  Proof.
+    revert n q.
+    depind p.
+    - intros. dependent destruction q; inv H; auto.
+    - intros. dependent destruction q; auto. cbn in H. apply IHp; auto.
+  Qed.
+
+  Lemma order_L_R {n} (i : fin n) :
+    order i (L_R 1 i) = EQ.
+  Proof.
+    induction i; auto.
+  Qed.
+
+  Lemma order_FS {n} (i : fin n) :
+    order i (FS i) = LT.
+  Proof.
+    induction i; auto.
+  Qed.
+
+  (* Lemma order_FS' {n} (i : fin n) : *)
+  (*   order (FS i) i = g. *)
+  (* Proof. *)
+  (*   apply order_flip; apply order_FS. *)
+  (* Qed. *)
+
+  Lemma order_FS_g {m n} (p : fin m) (q : fin n) :
+    order (FS p) q = GT ->
+    order p q = EQ \/ order p q = GT.
+  Proof.
+    intros. generalize dependent n. depind p; intros.
+    - dependent destruction q.
+      + left; auto.
+      + dependent destruction q; inv H.
+    - dependent destruction q.
+      + right; auto.
+      + cbn in H. destruct (IHp _ q H); auto.
+  Qed.
+
+  Lemma order_cases {m n} (p : fin m) (q : fin n) :
+    order p q = LT \/ order p q = EQ \/ order p q = GT.
+  Proof.
+    destruct (order p q); intuition.
+  Qed.
+
+  Lemma order_cases' {m n} (p : fin m) (q : fin n) :
+    {order p q = LT} + {order p q = EQ} + {order p q = GT}.
+  Proof.
+    destruct (order p q); intuition.
+  Qed.
+
+  Lemma ltb_L_R m n (p : fin m) (q : fin n) : order p q = order (L_R 1 p) q.
+  Proof.
+    intros. revert n q. depind p.
+    - reflexivity.
+    - dependent destruction q.
+      + reflexivity.
+      + cbn. rewrite IHp. reflexivity.
+  Qed.
+
+
+  (* p is not the highest possible value, so it can be seen as a value of type fin (S n) *)
+  (* Equations cons_vec {n : nat} (t : thread) (v : vec n) : vec (S n) := *)
+  (*   cons_vec t v F1      := t; *)
+  (*   cons_vec t v (FS i)  := v i. *)
+  (* Transparent cons_vec. *)
+
+  Equations not_highest {n} (p q : fin (S (S n))) (H: order p q = LT) : fin (S n) :=
+    not_highest F1 q H := F1 ;
+    not_highest (FS p') F1 H := _;
+    @not_highest 0 (FS p') (FS q') H := _;
+    @not_highest (S n) (FS p') (FS q') H := FS (not_highest p' q' _).
+  Next Obligation.
+    intros. inv H.
+  Defined.
+  Next Obligation.
+    intros. cbn in *. dependent destruction p'. 2: inv p'.
+    dependent destruction q'. inv H. inv q'.
+  Defined.
+  Next Obligation.
+    auto.
+  Defined.
+
+  (* Definition not_highest {n} (p q : fin (S (S n))) (H: order p q = l) : fin (S n). *)
+  (*   remember (S n). remember (S n0). revert n n0 Heqn0 Heqn1 H. *)
+  (*   (* depind p. *) *)
+  (*   induction p; intros; subst; auto. *)
+  (*   - subst. apply F1. *)
+  (*   - (* remember (S n). destruct q. inv H. *) *)
+  (*     (* subst. apply FS. destruct n. *) *)
+  (*     (* + cbn in H. depind p. depind q. inv H. inv IHq. *) *)
+
+  (*     (* inv Heqn1. eapply IHp; eauto. *) *)
+
+  (*     destruct n. *)
+  (*     + cbn in H. Show Proof. *)
+  (*       remember (S n0). *)
+  (*       destruct q; inv H; auto. inv Heqn1. eapply IHp; eauto. *)
+  (*       (* dependent destruction q; inv H. Show Proof. eapply IHp; eauto. *) *)
+  (*       (* dependent destruction p; dependent destruction q; inv H1; inv q. *) *)
+  (*     + Show Proof. simpl in H. remember (S n0). destruct q. inv H. *)
+  (*       inv Heqn1. eapply IHp; eauto. *)
+  (* Defined. *)
+
+  (* not used *)
+  Lemma not_highest_FS {n} (p q : fin (S (S n))) H H' :
+    (not_highest (FS p) (FS q) H) = FS (not_highest p q H').
+  Proof.
+    simp not_highest. f_equal. f_equal. apply proof_irrelevance.
+  Qed.
+
+  Lemma order_not_highest_equal {n} (p q r : fin (S (S n))) H :
+    order p r = order (not_highest p q H) r.
+  Proof.
+    depind p.
+    - simp not_highest. reflexivity.
+    - dependent destruction q. inv H.
+      destruct n.
+      + cbn in *. depind p. depind q. inv H. inv q. inv p.
+      + cbn in H. rewrite not_highest_FS with (H':=H).
+        cbn in *. dependent destruction r; auto.
+  Qed.
+
+  Lemma order_not_highest {n} (p q : fin (S (S n))) H :
+    order (not_highest p q H) p = EQ.
+  Proof.
+    depind p; auto.
+    - simp not_highest. auto.
+    - dependent destruction q. inv H.
+      destruct n.
+      + cbn in H.
+        dependent destruction p. 2: inv p.
+        dependent destruction q. inv H. inv q.
+      + simp not_highest. cbn. apply IHp; auto.
+  Qed.
+
+  (* view a [fin n] as a [fin (S n)] *)
+  Equations fin_S {n} (i : fin n) : fin (S n) :=
+    fin_S F1 := F1;
+    fin_S (FS i') := FS (fin_S i').
+  (* Proof. *)
+  (*   depind i. *)
+  (*   - apply F1. *)
+  (*   - apply FS. apply IHi. *)
+  (* Defined. *)
+
+  (* Lemma fin_S_not_highest *)
+
+  Lemma order_fin_S_equal {n} (i : fin n) : order i (fin_S i) = EQ.
+  Proof.
+    depind i; auto.
+  Qed.
+
+  Lemma order_fin_S m n (p : fin m) (q : fin n) : order p q = order (fin_S p) q.
+  Proof.
+    intros. revert n q. depind p.
+    - reflexivity.
+    - dependent destruction q.
+      + reflexivity.
+      + cbn. rewrite IHp. reflexivity.
+  Qed.
+
+  Lemma fin_S_not_highest {n} (p q : fin (S (S n))) H : fin_S (not_highest p q H) = p.
+  Proof.
+    depind p; cbn; auto.
+    - simp not_highest. simp fin_S. reflexivity.
+    - dependent destruction q. inv H.
+      destruct n. cbn in H.
+      dependent destruction p. dependent destruction q. inv H. inv q. inv p.
+      simp not_highest. simp fin_S. f_equal. apply IHp; auto.
+  Qed.
+
+  Lemma not_highest_fin_S {n} (p : fin (S n)) q H : (not_highest (fin_S p) q H) = p.
+  Proof.
+    destruct n.
+    { dependent destruction p. auto. inv p. }
+    depind p; auto.
+    dependent destruction q. inv H.
+    revert H. simp fin_S. intro.
+    destruct n; auto.
+    - cbn in *. dependent destruction p. 2: inv p. auto.
+    - simp not_highest. f_equal. auto.
+  Qed.
+
+  (* p is greater than another value, so we can subtract one *)
+  Equations subtract_one {n} (p q : fin (S n)) (H: order p q = GT) : fin n :=
+  subtract_one F1 q H := _;
+  subtract_one (FS p') q H := p'.
+  Next Obligation.
+    intros. dependent destruction q; inv H.
+  Defined.
+
+  Lemma subtract_one_FS {n} p (q : fin (S n)) H :
+    subtract_one (FS p) q H = p.
+  Proof.
+    reflexivity.
+  Qed.
+
+  Lemma FS_subtract_one {n} (p q : fin (S n)) H :
+    FS (subtract_one p q H) = p.
+  Proof.
+    dependent destruction p.
+    - dependent destruction q; inv H.
+    - reflexivity.
+  Qed.
+
+  Lemma subtract_one_order {n} (p q : fin (S n)) (H : order p q = GT) :
+    order p (subtract_one p q H) = GT.
+  Proof.
+    dependent destruction p.
+    - dependent destruction q; inv H.
+    - destruct n. inv p. rewrite subtract_one_FS. apply order_flip. apply order_FS.
+  Qed.
+
+  Lemma subtract_one_order_g {n} (p q r : fin (S n)) H :
+    order p q = GT ->
+    order (subtract_one p r H) q = EQ \/ order (subtract_one p r H) q = GT.
+  Proof.
+    intros.
+    dependent destruction p.
+    - dependent destruction q; inv H0.
+    - destruct n. inv p.
+      rewrite subtract_one_FS. apply order_FS_g; auto.
+  Qed.
+
+  Lemma subtract_one_l {n} (p q r : fin (S n)) H :
+     order (subtract_one p r H) q = LT ->
+     order p q = EQ \/ order p q = LT.
+  Proof.
+    intros.
+    depind p. dependent destruction r; inv H.
+    destruct n. inv p. specialize (IHp n p eq_refl JMeq_refl).
+    rewrite subtract_one_FS in H0.
+    dependent destruction q. dependent destruction p; inv H0. cbn.
+    dependent destruction p. dependent destruction q; auto.
+    cbn in H0.
+    eapply (IHp q (fin_S p) _ _). Unshelve.
+    - rewrite <- order_flip. rewrite <- order_fin_S. apply order_FS.
+    - rewrite subtract_one_FS. auto.
+  Qed.
+
+  Lemma remove_vec_index_before' {n} (v : vec (S n)) i j
+    (Hj : order j i = LT) :
+    v (fin_S j) = remove_vec v i j.
+  Proof.
+    revert v j Hj. depind i; intros; auto. dependent destruction j; inv Hj.
+    destruct n. inv j. dependent destruction j; auto. cbn. simp fin_S.
+    erewrite <- IHi; auto.
+  Qed.
+
+  (* after the element removed, we need to subtract one from the index *)
+  Lemma remove_vec_index_after' {n} (v : vec (S n)) i j
+        (Hj : order j i = GT) :
+    v (FS j) = remove_vec v i j.
+  Proof.
+    revert v i Hj. depind j; intros. dependent destruction i; auto; inv Hj.
+    dependent destruction i.
+    - destruct n. inv j. reflexivity.
+    - destruct n. inv j. cbn in *. rewrite <- IHj; auto.
+  Qed.
+
+  (* at the element removed, we also subtract one. TODO: can we unify this with prev lemma? *)
+  Lemma remove_vec_index_eq' {n} (v : vec (S n)) i j
+        (Hj : order j i = EQ) :
+    v (FS j) = remove_vec v i j.
+  Proof.
+    revert v i Hj. depind j; intros. dependent destruction i; auto; inv Hj.
+    dependent destruction i. inv Hj.
+    destruct n. inv j. cbn in *. rewrite <- IHj; auto.
+  Qed.
+
+  Require Import Coq.Logic.FinFun.
+  (* Require Import Coq.Classes.Morphisms. *)
+
+  (* why.. *)
+  Instance test: subrelation eq (flip impl).
+  Proof.
+    repeat intro. subst. auto.
+  Qed.
+
+  (* Definition remove_at_permutation {n} (p : fin (S (S n)) -> fin (S (S n))) *)
+  (*            (r : fin (S (S n))) *)
+  (*            (Hp : Injective p) *)
+  (*   : fin (S n) -> fin (S n). *)
+  (*   intro i. *)
+  (*   destruct (order_cases' i r) as [[Hi | Hi] | Hi]. *)
+  (*   - (* i < r *) *)
+  (*     remember (p (fin_S i)) as pi. *)
+  (*     destruct (order_cases' pi r) as [[Hpi | Hpi] | Hpi]. *)
+  (*     + (* p i < r *) *)
+  (*       apply (not_highest _ _ Hpi). *)
+  (*     + (* p i = r, return p (p i) *) *)
+  (*       remember (p pi) as ppi. *)
+  (*       destruct (order_cases' ppi r) as [[Hppi | Hppi] | Hppi]. *)
+  (*       * apply (not_highest _ _ Hppi). *)
+  (*       * (* impossible since p should be an injection: p i = r = p (p i), but i < p i *) *)
+  (*         apply order_eq in Hpi, Hppi. subst. apply Hp in Hppi. rewrite Hppi in Hi. *)
+  (*         rewrite order_fin_S_equal in Hi. inv Hi. *)
+  (*       * apply (subtract_one _ _ Hppi). *)
+  (*     + (* p i > r *) *)
+  (*       apply (subtract_one _ _ Hpi). *)
+  (*   - apply F1. *)
+  (*   - apply F1. *)
+  (* Defined. *)
+
+  Definition remove_at_permutation {n} (p : fin (S (S n)) -> fin (S (S n)))
+             (r : fin (S (S n)))
+             (Hp : Injective p)
+    :
+    { p' : (fin (S n) -> fin (S n)) &
+             (forall i, match (order_cases' i r) with
+                   | inleft (left Hi) =>
+                       (* i < r *)
+                       let pi := p (fin_S i) in
+                       match (order_cases' pi r) with
+                       | inleft (left Hpi) => (* p i < r *)
+                           p' i = not_highest _ _ Hpi
+                       | inleft (right Hpi) => (* p i = r *)
+                           let ppi := p pi in
+                           match (order_cases' ppi r) with
+                           | inleft (left Hppi) =>
+                               p' i = not_highest _ _ Hppi
+                           | inleft (right Hppi) => False
+                           | inright Hppi =>
+                               p' i = subtract_one _ _ Hppi
+                           end
+                       | inright Hpi => (* p i > r *)
+                           p' i = subtract_one _ _ Hpi
+                       end
+                   | _(* inleft (right Hi) *) =>
+                       (* i >= r *)
+                       let pi := p (FS i) in
+                       match (order_cases' pi r) with
+                       | inleft (left Hpi) => (* p (i + 1) < r *)
+                           p' i = not_highest _ _ Hpi
+                       | inleft (right Hpi) => (* p (i + 1) = r *)
+                           let ppi := p pi in
+                           match (order_cases' ppi r) with
+                           | inleft (left Hppi) =>
+                               p' i = not_highest _ _ Hppi
+                           | inleft (right Hppi) => False
+                           | inright Hppi =>
+                               p' i = subtract_one _ _ Hppi
+                           end
+                       | inright Hpi => (* p (i + 1) > r *)
+                           p' i = subtract_one _ _ Hpi
+                       end
+                   (* | inright Hi => *)
+                   (*     (* i > r *) *)
+                   (*     let pi := p (FS i) in *)
+                   (*     match (order_cases' pi r) with *)
+                   (*     | inleft (left Hpi) => (* p i < r *) *)
+                   (*         p' i = not_highest _ _ Hpi *)
+                   (*     | inleft (right Hpi) => (* p i = r *) *)
+                   (*         let ppi := p pi in *)
+                   (*         match (order_cases' ppi r) with *)
+                   (*         | inleft (left Hppi) => *)
+                   (*             p' i = not_highest _ _ Hppi *)
+                   (*         | inleft (right Hppi) => False *)
+                   (*         | inright Hppi => *)
+                   (*             p' i = subtract_one _ _ Hppi *)
+                   (*         end *)
+                   (*     | inright Hpi => (* p i > r *) *)
+                   (*         p' i = subtract_one _ _ Hpi *)
+                   (*     end *)
+                   end)
+    }.
+  Proof.
+    eexists. Unshelve.
+    2: {
+      intro i.
+      destruct (order_cases' i r) as [[Hi | Hi] | Hi].
+      - (* i < r *)
+        remember (p (fin_S i)) as pi.
+        destruct (order_cases' pi r) as [[Hpi | Hpi] | Hpi].
+        + (* p i < r *)
+          apply (not_highest _ _ Hpi).
+        + (* p i = r, return p (p i) *)
+          remember (p pi) as ppi.
+          destruct (order_cases' ppi r) as [[Hppi | Hppi] | Hppi].
+          * apply (not_highest _ _ Hppi).
+          * (* impossible since p should be an injection: p i = r = p (p i), but i < p i *)
+            apply order_eq in Hpi, Hppi. subst. apply Hp in Hppi. rewrite Hppi in Hi.
+            rewrite order_fin_S_equal in Hi. inv Hi.
+          * apply (subtract_one _ _ Hppi).
+        + (* p i > r *)
+          apply (subtract_one _ _ Hpi).
+      - (* i = r *)
+        remember (p (FS i)) as pi.
+        destruct (order_cases' pi r) as [[Hpi | Hpi] | Hpi].
+        + (* p (i + 1) < r *)
+          apply (not_highest _ _ Hpi).
+        + (* p (i + 1) = r, return p (p (i + 1)) *)
+          remember (p pi) as ppi.
+          destruct (order_cases' ppi r) as [[Hppi | Hppi] | Hppi].
+          * apply (not_highest _ _ Hppi).
+          * (* impossible since p should be an injection:
+               p (i + 1) = r = p (p (i + 1)), but i = r < i + 1 *)
+            apply order_eq in Hpi, Hppi. subst. apply Hp in Hppi. rewrite Hppi in Hi.
+            rewrite order_FS in Hi. inv Hi.
+          * apply (subtract_one _ _ Hppi).
+        + (* p i > r *)
+          apply (subtract_one _ _ Hpi).
+      - (* i > r *)
+        remember (p (FS i)) as pi.
+        destruct (order_cases' pi r) as [[Hpi | Hpi] | Hpi].
+        + (* p (i + 1) < r *)
+          apply (not_highest _ _ Hpi).
+        + (* p (i + 1) = r, return p (p (i + 1)) *)
+          remember (p pi) as ppi.
+          destruct (order_cases' ppi r) as [[Hppi | Hppi] | Hppi].
+          * apply (not_highest _ _ Hppi).
+          * (* impossible since p should be an injection:
+               p (i + 1) = r = p (p (i + 1)), but i > r -> i + 1 > r *)
+            apply order_eq in Hpi, Hppi. subst. apply Hp in Hppi. rewrite Hppi in Hi.
+            rewrite order_FS in Hi. inv Hi.
+          * apply (subtract_one _ _ Hppi).
+        + (* p i > r *)
+          apply (subtract_one _ _ Hpi).
+    }
+    intro i. cbn.
+    (* remember (order i r). *)
+    (* dependent destruction (order_cases i r)). *)
+    destruct (order_cases' i r) as [[Hi | Hi] | Hi].
+    - (* i < r *)
+      set (pi := p (fin_S i)).
+      destruct (order_cases' pi r) as [[Hpi | Hpi] | Hpi]; auto.
+      (* p i = r *)
+      set (ppi := p pi).
+      destruct (order_cases' ppi r) as [[Hppi | Hppi] | Hppi]; auto.
+      (* p p i = r, contradiction *)
+      apply order_eq in Hpi, Hppi. subst. apply Hp in Hppi. rewrite Hppi in Hi.
+      rewrite order_fin_S_equal in Hi. inv Hi.
+    - (* i = r *)
+      set (pi := p (FS i)).
+      destruct (order_cases' pi r) as [[Hpi | Hpi] | Hpi]; auto.
+      (* p i = r *)
+      set (ppi := p pi).
+      destruct (order_cases' ppi r) as [[Hppi | Hppi] | Hppi]; auto.
+      (* p p i = r, contradiction *)
+      apply order_eq in Hpi, Hppi. subst. apply Hp in Hppi. rewrite Hppi in Hi.
+      rewrite order_FS in Hi. inv Hi.
+    - (* i > r *)
+      set (pi := p (FS i)).
+      destruct (order_cases' pi r) as [[Hpi | Hpi] | Hpi]; auto.
+      (* p i = r *)
+      set (ppi := p pi).
+      destruct (order_cases' ppi r) as [[Hppi | Hppi] | Hppi]; auto.
+      (* p p i = r, contradiction *)
+      apply order_eq in Hpi, Hppi. subst. apply Hp in Hppi. rewrite Hppi in Hi.
+      rewrite order_FS in Hi. inv Hi.
+  Qed.
+
+  Lemma bijective_injective {n} (p q : fin n -> fin n)
+        (Hqp: forall i, q (p i) = i) :
+    Injective p.
+  Proof.
+    intros i1 i2 ?. apply (f_equal q) in H. do 2 rewrite Hqp in H. auto.
+  Qed.
+
+  Lemma remove_at_permutation_correct {n} (p q : fin (S (S n)) -> fin (S (S n))) r
+        (Hpq : forall i, p (q i) = i)
+        (Hqp : forall i, q (p i) = i) :
+    let p' := projT1 (remove_at_permutation p r (bijective_injective _ _ Hqp)) in
+    let q' := projT1 (remove_at_permutation q r (bijective_injective _ _ Hpq)) in
+    (forall i, p' (q' i) = i) /\ (forall i, q' (p' i) = i).
+  Proof.
+    destruct (remove_at_permutation p r _) as (p' & Hp).
+    destruct (remove_at_permutation q r _) as (q' & Hq).
+    cbn in *. split.
+    {
+      intro i.
+      specialize (Hq i).
+      destruct (order_cases' i r) as [[Hi | Hi] | Hi].
+      - (* i < r *)
+        destruct (order_cases' (q (fin_S i)) r) as [[Hqi | Hqi] | Hqi].
+        + (* q i < r *)
+          rewrite Hq. specialize (Hp (q' i)). rewrite Hq in Hp.
+          rewrite fin_S_not_highest in Hp. rewrite Hpq in Hp.
+          destruct (order_cases' (not_highest (q (fin_S i)) r Hqi) r) as [[Hqi' | Hqi'] | Hqi'].
+          2, 3: erewrite <- order_not_highest_equal in Hqi'; rewrite Hqi in Hqi'; inv Hqi'.
+          destruct (order_cases' (fin_S i) r) as [[Hi' | Hi'] | Hi'].
+          2, 3: rewrite order_fin_S in Hi; rewrite Hi' in Hi; inv Hi.
+          rewrite Hp. rewrite not_highest_fin_S. reflexivity.
+        + (* q i = r, so we apply q again *)
+          destruct (order_cases' (q (q (fin_S i))) r) as [[Hqqi | Hqqi] | Hqqi].
+          * (* q (q i) < r *)
+            rewrite Hq. specialize (Hp (q' i)). rewrite Hq in Hp.
+            rewrite fin_S_not_highest in Hp. do 2 rewrite Hpq in Hp.
+            destruct (order_cases' (not_highest (q (q (fin_S i))) r Hqqi) r) as
+              [[Hqqi' | Hqqi'] | Hqqi'].
+            2, 3: erewrite <- order_not_highest_equal in Hqqi'; rewrite Hqqi in Hqqi'; inv Hqqi'.
+            destruct (order_cases' (q (fin_S i)) r) as [[Hqi' | Hqi'] | Hqi'].
+            1, 3: rewrite Hqi' in Hqi; inv Hqi.
+            destruct (order_cases' (fin_S i) r) as [[Hi' | Hi'] | Hi'].
+            2, 3: rewrite order_fin_S in Hi; rewrite Hi' in Hi; inv Hi.
+            rewrite Hp. rewrite not_highest_fin_S. reflexivity.
+          * (* q (q i) = r *)
+            contradiction.
+          * (* q (q i) > r *)
+            rewrite Hq. specialize (Hp (q' i)). rewrite Hq in Hp.
+            rewrite FS_subtract_one in Hp. do 2 rewrite Hpq in Hp.
+            destruct (order_cases' (subtract_one (q (q (fin_S i))) r Hqqi) r) as
+              [[Hqqis | Hqqis] | Hqqis].
+            -- (* q (q i) - 1 < r *)
+              (* contradiction *)
+              apply (subtract_one_l) in Hqqis.
+              destruct Hqqis as [Hqqis | Hqqis]; rewrite Hqqi in Hqqis; inv Hqqis.
+            -- (* q (q i) - 1 = r *)
+              destruct (order_cases' (q (fin_S i)) r) as [[Hqi' | Hqi'] | Hqi'].
+              1, 3: rewrite Hqi' in Hqi; inv Hqi. clear Hqi'.
+              destruct (order_cases' (fin_S i) r) as [[Hi' | Hi'] | Hi'].
+              2, 3: rewrite order_fin_S in Hi; rewrite Hi' in Hi; inv Hi.
+              rewrite Hp. rewrite not_highest_fin_S. reflexivity.
+            -- (* q (q i) - 1 > r, same as above *)
+              destruct (order_cases' (q (fin_S i)) r) as [[Hqi' | Hqi'] | Hqi'].
+              1, 3: rewrite Hqi' in Hqi; inv Hqi. clear Hqi'.
+              destruct (order_cases' (fin_S i) r) as [[Hi' | Hi'] | Hi'].
+              2, 3: rewrite order_fin_S in Hi; rewrite Hi' in Hi; inv Hi.
+              rewrite Hp. rewrite not_highest_fin_S. reflexivity.
+        + (* q i > r *)
+          rewrite Hq. specialize (Hp (q' i)). rewrite Hq in Hp.
+          rewrite FS_subtract_one in Hp. rewrite Hpq in Hp.
+          destruct (order_cases' (subtract_one (q (fin_S i)) r Hqi) r) as
+            [[Hqis | Hqis] | Hqis].
+          * (* q i - 1 < r *)
+            (* contradiction *)
+            apply (subtract_one_l) in Hqis.
+            destruct Hqis as [Hqis | Hqis]; rewrite Hqi in Hqis; inv Hqis.
+          * (* q i - 1 = r *)
+            destruct (order_cases' (fin_S i) r) as [[Hi' | Hi'] | Hi'].
+            2, 3: rewrite order_fin_S in Hi; rewrite Hi' in Hi; inv Hi.
+            rewrite Hp. rewrite not_highest_fin_S. reflexivity.
+          * (* q i - 1 > r *)
+            destruct (order_cases' (fin_S i) r) as [[Hi' | Hi'] | Hi'].
+            2, 3: rewrite order_fin_S in Hi; rewrite Hi' in Hi; inv Hi.
+            rewrite Hp. rewrite not_highest_fin_S. reflexivity.
+      - (* i = r *)
+        destruct (order_cases' (q (FS i)) r) as [[Hqi | Hqi] | Hqi].
+        + (* q (i + 1) < r *)
+          rewrite Hq. specialize (Hp (q' i)). rewrite Hq in Hp.
+          rewrite fin_S_not_highest in Hp. rewrite Hpq in Hp.
+          destruct (order_cases' (not_highest (q (FS i)) r Hqi) r) as [[Hqi' | Hqi'] | Hqi'].
+          2, 3: erewrite <- order_not_highest_equal in Hqi'; rewrite Hqi in Hqi'; inv Hqi'.
+          destruct (order_cases' (FS i) r) as [[Hi' | Hi'] | Hi'].
+          1, 2: apply order_e_FS in Hi; rewrite Hi' in Hi; inv Hi.
+          rewrite Hp. rewrite subtract_one_FS. reflexivity.
+        + (* q (i + 1) = r *)
+          destruct (order_cases' (q (q (FS i))) r) as [[Hqqi | Hqqi] | Hqqi].
+          * (* q (q (i + 1)) < r *)
+            rewrite Hq. specialize (Hp (q' i)). rewrite Hq in Hp.
+            rewrite fin_S_not_highest in Hp. do 2 rewrite Hpq in Hp.
+            destruct (order_cases' (not_highest (q (q (FS i))) r Hqqi) r) as
+              [[Hqqi' | Hqqi'] | Hqqi'].
+            2, 3: erewrite <- order_not_highest_equal in Hqqi'; rewrite Hqqi in Hqqi'; inv Hqqi'.
+            destruct (order_cases' (q (FS i)) r) as [[Hqi' | Hqi'] | Hqi'].
+            1, 3: rewrite Hqi' in Hqi; inv Hqi.
+            destruct (order_cases' (FS i) r) as [[Hio | Hio] | Hio].
+            { apply order_e_FS in Hi. rewrite Hio in Hi. inv Hi. }
+            { contradiction. }
+            rewrite Hp. rewrite subtract_one_FS. reflexivity.
+          * (* q (q (i + 1)) = r *)
+            contradiction.
+          * (* q (q (i + 1)) > r *)
+            rewrite Hq. specialize (Hp (q' i)). rewrite Hq in Hp.
+            rewrite FS_subtract_one in Hp. do 2 rewrite Hpq in Hp.
+            destruct (order_cases' (subtract_one (q (q (FS i))) r Hqqi) r) as
+              [[Hqqis | Hqqis] | Hqqis].
+            -- (* (q (q (i + 1))) - 1 < r *)
+              apply (subtract_one_l) in Hqqis.
+              destruct Hqqis as [Hqqis | Hqqis]; rewrite Hqqi in Hqqis; inv Hqqis.
+            -- (* (q (q (i + 1))) - 1 = r *)
+              destruct (order_cases' (q (FS i)) r) as [[Hqi' | Hqi'] | Hqi'].
+              1, 3: rewrite Hqi' in Hqi; inv Hqi. clear Hqi'.
+              destruct (order_cases' (FS i) r) as [[Hi' | Hi'] | Hi'].
+              { apply order_e_FS in Hi. rewrite Hi' in Hi. inv Hi. }
+              { contradiction. }
+              rewrite Hp. rewrite subtract_one_FS. reflexivity.
+            -- (* (q (q (i + 1))) - 1 > r *)
+              destruct (order_cases' (q (FS i)) r) as [[Hqi' | Hqi'] | Hqi'].
+              1, 3: rewrite Hqi' in Hqi; inv Hqi. clear Hqi'.
+              destruct (order_cases' (FS i) r) as [[Hi' | Hi'] | Hi'].
+              { apply order_e_FS in Hi. rewrite Hi' in Hi. inv Hi. }
+              { contradiction. }
+              rewrite Hp. rewrite subtract_one_FS. reflexivity.
+        + (* q (i + 1) > r *)
+          rewrite Hq. specialize (Hp (q' i)). rewrite Hq in Hp.
+          rewrite FS_subtract_one in Hp. rewrite Hpq in Hp.
+          destruct (order_cases' (subtract_one (q (FS i)) r Hqi) r) as
+            [[Hqis | Hqis] | Hqis].
+          * (* (q (i + 1)) - 1 < r *)
+            (* contradiction *)
+            apply subtract_one_l in Hqis.
+            destruct Hqis as [Hqis | Hqis]; rewrite Hqi in Hqis; inv Hqis.
+          * (* (q (i + 1)) - 1 = r *)
+            destruct (order_cases' (FS i) r) as [[Hi' | Hi'] | Hi'].
+            1, 2: apply order_e_FS in Hi; rewrite Hi' in Hi; inv Hi.
+            rewrite Hp. rewrite subtract_one_FS. reflexivity.
+          * (* (q (i + 1)) - 1 > r *)
+            destruct (order_cases' (FS i) r) as [[Hi' | Hi'] | Hi'].
+            1, 2: apply order_e_FS in Hi; rewrite Hi' in Hi; inv Hi.
+            rewrite Hp. rewrite subtract_one_FS. reflexivity.
+      - (* i > r *)
+        (* exactly the same as prev case *)
+        destruct (order_cases' (q (FS i)) r) as [[Hqi | Hqi] | Hqi].
+        + (* q (i + 1) < r *)
+          rewrite Hq. specialize (Hp (q' i)). rewrite Hq in Hp.
+          rewrite fin_S_not_highest in Hp. rewrite Hpq in Hp.
+          destruct (order_cases' (not_highest (q (FS i)) r Hqi) r) as [[Hqi' | Hqi'] | Hqi'].
+          2, 3: erewrite <- order_not_highest_equal in Hqi'; rewrite Hqi in Hqi'; inv Hqi'.
+          destruct (order_cases' (FS i) r) as [[Hi' | Hi'] | Hi'].
+          1, 2: apply order_g_FS in Hi; rewrite Hi' in Hi; inv Hi.
+          rewrite Hp. rewrite subtract_one_FS. reflexivity.
+        + (* q (i + 1) = r *)
+          destruct (order_cases' (q (q (FS i))) r) as [[Hqqi | Hqqi] | Hqqi].
+          * (* q (q (i + 1)) < r *)
+            rewrite Hq. specialize (Hp (q' i)). rewrite Hq in Hp.
+            rewrite fin_S_not_highest in Hp. do 2 rewrite Hpq in Hp.
+            destruct (order_cases' (not_highest (q (q (FS i))) r Hqqi) r) as
+              [[Hqqi' | Hqqi'] | Hqqi'].
+            2, 3: erewrite <- order_not_highest_equal in Hqqi'; rewrite Hqqi in Hqqi'; inv Hqqi'.
+            destruct (order_cases' (q (FS i)) r) as [[Hqi' | Hqi'] | Hqi'].
+            1, 3: rewrite Hqi' in Hqi; inv Hqi.
+            destruct (order_cases' (FS i) r) as [[Hio | Hio] | Hio].
+            { apply order_g_FS in Hi. rewrite Hio in Hi. inv Hi. }
+            { contradiction. }
+            rewrite Hp. rewrite subtract_one_FS. reflexivity.
+          * (* q (q (i + 1)) = r *)
+            contradiction.
+          * (* q (q (i + 1)) > r *)
+            rewrite Hq. specialize (Hp (q' i)). rewrite Hq in Hp.
+            rewrite FS_subtract_one in Hp. do 2 rewrite Hpq in Hp.
+            destruct (order_cases' (subtract_one (q (q (FS i))) r Hqqi) r) as
+              [[Hqqis | Hqqis] | Hqqis].
+            -- (* (q (q (i + 1))) - 1 < r *)
+              apply (subtract_one_l) in Hqqis.
+              destruct Hqqis as [Hqqis | Hqqis]; rewrite Hqqi in Hqqis; inv Hqqis.
+            -- (* (q (q (i + 1))) - 1 = r *)
+              destruct (order_cases' (q (FS i)) r) as [[Hqi' | Hqi'] | Hqi'].
+              1, 3: rewrite Hqi' in Hqi; inv Hqi. clear Hqi'.
+              destruct (order_cases' (FS i) r) as [[Hi' | Hi'] | Hi'].
+              { apply order_g_FS in Hi. rewrite Hi' in Hi. inv Hi. }
+              { contradiction. }
+              rewrite Hp. rewrite subtract_one_FS. reflexivity.
+            -- (* (q (q (i + 1))) - 1 > r *)
+              destruct (order_cases' (q (FS i)) r) as [[Hqi' | Hqi'] | Hqi'].
+              1, 3: rewrite Hqi' in Hqi; inv Hqi. clear Hqi'.
+              destruct (order_cases' (FS i) r) as [[Hi' | Hi'] | Hi'].
+              { apply order_g_FS in Hi. rewrite Hi' in Hi. inv Hi. }
+              { contradiction. }
+              rewrite Hp. rewrite subtract_one_FS. reflexivity.
+        + (* q (i + 1) > r *)
+          rewrite Hq. specialize (Hp (q' i)). rewrite Hq in Hp.
+          rewrite FS_subtract_one in Hp. rewrite Hpq in Hp.
+          destruct (order_cases' (subtract_one (q (FS i)) r Hqi) r) as
+            [[Hqis | Hqis] | Hqis].
+          * (* (q (i + 1)) - 1 < r *)
+            (* contradiction *)
+            apply subtract_one_l in Hqis.
+            destruct Hqis as [Hqis | Hqis]; rewrite Hqi in Hqis; inv Hqis.
+          * (* (q (i + 1)) - 1 = r *)
+            destruct (order_cases' (FS i) r) as [[Hi' | Hi'] | Hi'].
+            1, 2: apply order_g_FS in Hi; rewrite Hi' in Hi; inv Hi.
+            rewrite Hp. rewrite subtract_one_FS. reflexivity.
+          * (* (q (i + 1)) - 1 > r *)
+            destruct (order_cases' (FS i) r) as [[Hi' | Hi'] | Hi'].
+            1, 2: apply order_g_FS in Hi; rewrite Hi' in Hi; inv Hi.
+            rewrite Hp. rewrite subtract_one_FS. reflexivity.
+    }
+    {
+      intro i.
+      specialize (Hp i).
+      destruct (order_cases' i r) as [[Hi | Hi] | Hi].
+      - (* i < r *)
+        destruct (order_cases' (p (fin_S i)) r) as [[Hpi | Hpi] | Hpi].
+        + (* p i < r *)
+          rewrite Hp. specialize (Hq (p' i)). rewrite Hp in Hq.
+          rewrite fin_S_not_highest in Hq. rewrite Hqp in Hq.
+          destruct (order_cases' (not_highest (p (fin_S i)) r Hpi) r) as [[Hpi' | Hpi'] | Hpi'].
+          2, 3: erewrite <- order_not_highest_equal in Hpi'; rewrite Hpi in Hpi'; inv Hpi'.
+          destruct (order_cases' (fin_S i) r) as [[Hi' | Hi'] | Hi'].
+          2, 3: rewrite order_fin_S in Hi; rewrite Hi' in Hi; inv Hi.
+          rewrite Hq. rewrite not_highest_fin_S. reflexivity.
+        + (* p i = r, so we apply p again *)
+          destruct (order_cases' (p (p (fin_S i))) r) as [[Hppi | Hppi] | Hppi].
+          * (* p (p i) < r *)
+            rewrite Hp. specialize (Hq (p' i)). rewrite Hp in Hq.
+            rewrite fin_S_not_highest in Hq. do 2 rewrite Hqp in Hq.
+            destruct (order_cases' (not_highest (p (p (fin_S i))) r Hppi) r) as
+              [[Hppi' | Hppi'] | Hppi'].
+            2, 3: erewrite <- order_not_highest_equal in Hppi'; rewrite Hppi in Hppi'; inv Hppi'.
+            destruct (order_cases' (p (fin_S i)) r) as [[Hpi' | Hpi'] | Hpi'].
+            1, 3: rewrite Hpi' in Hpi; inv Hpi.
+            destruct (order_cases' (fin_S i) r) as [[Hi' | Hi'] | Hi'].
+            2, 3: rewrite order_fin_S in Hi; rewrite Hi' in Hi; inv Hi.
+            rewrite Hq. rewrite not_highest_fin_S. reflexivity.
+          * (* p (p i) = r *)
+            contradiction.
+          * (* p (p i) > r *)
+            rewrite Hp. specialize (Hq (p' i)). rewrite Hp in Hq.
+            rewrite FS_subtract_one in Hq. do 2 rewrite Hqp in Hq.
+            destruct (order_cases' (subtract_one (p (p (fin_S i))) r Hppi) r) as
+              [[Hppis | Hppis] | Hppis].
+            -- (* p (p i) - 1 < r *)
+              (* contradiction *)
+              apply (subtract_one_l) in Hppis.
+              destruct Hppis as [Hppis | Hppis]; rewrite Hppi in Hppis; inv Hppis.
+            -- (* p (p i) - 1 = r *)
+              destruct (order_cases' (p (fin_S i)) r) as [[Hpi' | Hpi'] | Hpi'].
+              1, 3: rewrite Hpi' in Hpi; inv Hpi. clear Hpi'.
+              destruct (order_cases' (fin_S i) r) as [[Hi' | Hi'] | Hi'].
+              2, 3: rewrite order_fin_S in Hi; rewrite Hi' in Hi; inv Hi.
+              rewrite Hq. rewrite not_highest_fin_S. reflexivity.
+            -- (* p (p i) - 1 > r, same as above *)
+              destruct (order_cases' (p (fin_S i)) r) as [[Hpi' | Hpi'] | Hpi'].
+              1, 3: rewrite Hpi' in Hpi; inv Hpi. clear Hpi'.
+              destruct (order_cases' (fin_S i) r) as [[Hi' | Hi'] | Hi'].
+              2, 3: rewrite order_fin_S in Hi; rewrite Hi' in Hi; inv Hi.
+              rewrite Hq. rewrite not_highest_fin_S. reflexivity.
+        + (* p i > r *)
+          rewrite Hp. specialize (Hq (p' i)). rewrite Hp in Hq.
+          rewrite FS_subtract_one in Hq. rewrite Hqp in Hq.
+          destruct (order_cases' (subtract_one (p (fin_S i)) r Hpi) r) as
+            [[Hpis | Hpis] | Hpis].
+          * (* p i - 1 < r *)
+            (* contradiction *)
+            apply (subtract_one_l) in Hpis.
+            destruct Hpis as [Hpis | Hpis]; rewrite Hpi in Hpis; inv Hpis.
+          * (* p i - 1 = r *)
+            destruct (order_cases' (fin_S i) r) as [[Hi' | Hi'] | Hi'].
+            2, 3: rewrite order_fin_S in Hi; rewrite Hi' in Hi; inv Hi.
+            rewrite Hq. rewrite not_highest_fin_S. reflexivity.
+          * (* p i - 1 > r *)
+            destruct (order_cases' (fin_S i) r) as [[Hi' | Hi'] | Hi'].
+            2, 3: rewrite order_fin_S in Hi; rewrite Hi' in Hi; inv Hi.
+            rewrite Hq. rewrite not_highest_fin_S. reflexivity.
+      - (* i = r *)
+        destruct (order_cases' (p (FS i)) r) as [[Hpi | Hpi] | Hpi].
+        + (* p (i + 1) < r *)
+          rewrite Hp. specialize (Hq (p' i)). rewrite Hp in Hq.
+          rewrite fin_S_not_highest in Hq. rewrite Hqp in Hq.
+          destruct (order_cases' (not_highest (p (FS i)) r Hpi) r) as [[Hpi' | Hpi'] | Hpi'].
+          2, 3: erewrite <- order_not_highest_equal in Hpi'; rewrite Hpi in Hpi'; inv Hpi'.
+          destruct (order_cases' (FS i) r) as [[Hi' | Hi'] | Hi'].
+          1, 2: apply order_e_FS in Hi; rewrite Hi' in Hi; inv Hi.
+          rewrite Hq. rewrite subtract_one_FS. reflexivity.
+        + (* p (i + 1) = r *)
+          destruct (order_cases' (p (p (FS i))) r) as [[Hppi | Hppi] | Hppi].
+          * (* p (p (i + 1)) < r *)
+            rewrite Hp. specialize (Hq (p' i)). rewrite Hp in Hq.
+            rewrite fin_S_not_highest in Hq. do 2 rewrite Hqp in Hq.
+            destruct (order_cases' (not_highest (p (p (FS i))) r Hppi) r) as
+              [[Hppi' | Hppi'] | Hppi'].
+            2, 3: erewrite <- order_not_highest_equal in Hppi'; rewrite Hppi in Hppi'; inv Hppi'.
+            destruct (order_cases' (p (FS i)) r) as [[Hpi' | Hpi'] | Hpi'].
+            1, 3: rewrite Hpi' in Hpi; inv Hpi.
+            destruct (order_cases' (FS i) r) as [[Hio | Hio] | Hio].
+            { apply order_e_FS in Hi. rewrite Hio in Hi. inv Hi. }
+            { contradiction. }
+            rewrite Hq. rewrite subtract_one_FS. reflexivity.
+          * (* p (p (i + 1)) = r *)
+            contradiction.
+          * (* p (p (i + 1)) > r *)
+            rewrite Hp. specialize (Hq (p' i)). rewrite Hp in Hq.
+            rewrite FS_subtract_one in Hq. do 2 rewrite Hqp in Hq.
+            destruct (order_cases' (subtract_one (p (p (FS i))) r Hppi) r) as
+              [[Hppis | Hppis] | Hppis].
+            -- (* (p (p (i + 1))) - 1 < r *)
+              apply (subtract_one_l) in Hppis.
+              destruct Hppis as [Hppis | Hppis]; rewrite Hppi in Hppis; inv Hppis.
+            -- (* (p (p (i + 1))) - 1 = r *)
+              destruct (order_cases' (p (FS i)) r) as [[Hpi' | Hpi'] | Hpi'].
+              1, 3: rewrite Hpi' in Hpi; inv Hpi. clear Hpi'.
+              destruct (order_cases' (FS i) r) as [[Hi' | Hi'] | Hi'].
+              { apply order_e_FS in Hi. rewrite Hi' in Hi. inv Hi. }
+              { contradiction. }
+              rewrite Hq. rewrite subtract_one_FS. reflexivity.
+            -- (* (p (p (i + 1))) - 1 > r *)
+              destruct (order_cases' (p (FS i)) r) as [[Hpi' | Hpi'] | Hpi'].
+              1, 3: rewrite Hpi' in Hpi; inv Hpi. clear Hpi'.
+              destruct (order_cases' (FS i) r) as [[Hi' | Hi'] | Hi'].
+              { apply order_e_FS in Hi. rewrite Hi' in Hi. inv Hi. }
+              { contradiction. }
+              rewrite Hq. rewrite subtract_one_FS. reflexivity.
+        + (* p (i + 1) > r *)
+          rewrite Hp. specialize (Hq (p' i)). rewrite Hp in Hq.
+          rewrite FS_subtract_one in Hq. rewrite Hqp in Hq.
+          destruct (order_cases' (subtract_one (p (FS i)) r Hpi) r) as
+            [[Hpis | Hpis] | Hpis].
+          * (* (p (i + 1)) - 1 < r *)
+            (* contradiction *)
+            apply subtract_one_l in Hpis.
+            destruct Hpis as [Hpis | Hpis]; rewrite Hpi in Hpis; inv Hpis.
+          * (* (p (i + 1)) - 1 = r *)
+            destruct (order_cases' (FS i) r) as [[Hi' | Hi'] | Hi'].
+            1, 2: apply order_e_FS in Hi; rewrite Hi' in Hi; inv Hi.
+            rewrite Hq. rewrite subtract_one_FS. reflexivity.
+          * (* (p (i + 1)) - 1 > r *)
+            destruct (order_cases' (FS i) r) as [[Hi' | Hi'] | Hi'].
+            1, 2: apply order_e_FS in Hi; rewrite Hi' in Hi; inv Hi.
+            rewrite Hq. rewrite subtract_one_FS. reflexivity.
+      - (* i > r *)
+        (* exactly the same as prev case *)
+        destruct (order_cases' (p (FS i)) r) as [[Hpi | Hpi] | Hpi].
+        + (* p (i + 1) < r *)
+          rewrite Hp. specialize (Hq (p' i)). rewrite Hp in Hq.
+          rewrite fin_S_not_highest in Hq. rewrite Hqp in Hq.
+          destruct (order_cases' (not_highest (p (FS i)) r Hpi) r) as [[Hpi' | Hpi'] | Hpi'].
+          2, 3: erewrite <- order_not_highest_equal in Hpi'; rewrite Hpi in Hpi'; inv Hpi'.
+          destruct (order_cases' (FS i) r) as [[Hi' | Hi'] | Hi'].
+          1, 2: apply order_g_FS in Hi; rewrite Hi' in Hi; inv Hi.
+          rewrite Hq. rewrite subtract_one_FS. reflexivity.
+        + (* p (i + 1) = r *)
+          destruct (order_cases' (p (p (FS i))) r) as [[Hppi | Hppi] | Hppi].
+          * (* p (p (i + 1)) < r *)
+            rewrite Hp. specialize (Hq (p' i)). rewrite Hp in Hq.
+            rewrite fin_S_not_highest in Hq. do 2 rewrite Hqp in Hq.
+            destruct (order_cases' (not_highest (p (p (FS i))) r Hppi) r) as
+              [[Hppi' | Hppi'] | Hppi'].
+            2, 3: erewrite <- order_not_highest_equal in Hppi'; rewrite Hppi in Hppi'; inv Hppi'.
+            destruct (order_cases' (p (FS i)) r) as [[Hpi' | Hpi'] | Hpi'].
+            1, 3: rewrite Hpi' in Hpi; inv Hpi.
+            destruct (order_cases' (FS i) r) as [[Hio | Hio] | Hio].
+            { apply order_g_FS in Hi. rewrite Hio in Hi. inv Hi. }
+            { contradiction. }
+            rewrite Hq. rewrite subtract_one_FS. reflexivity.
+          * (* p (p (i + 1)) = r *)
+            contradiction.
+          * (* p (p (i + 1)) > r *)
+            rewrite Hp. specialize (Hq (p' i)). rewrite Hp in Hq.
+            rewrite FS_subtract_one in Hq. do 2 rewrite Hqp in Hq.
+            destruct (order_cases' (subtract_one (p (p (FS i))) r Hppi) r) as
+              [[Hppis | Hppis] | Hppis].
+            -- (* (p (p (i + 1))) - 1 < r *)
+              apply (subtract_one_l) in Hppis.
+              destruct Hppis as [Hppis | Hppis]; rewrite Hppi in Hppis; inv Hppis.
+            -- (* (p (p (i + 1))) - 1 = r *)
+              destruct (order_cases' (p (FS i)) r) as [[Hpi' | Hpi'] | Hpi'].
+              1, 3: rewrite Hpi' in Hpi; inv Hpi. clear Hpi'.
+              destruct (order_cases' (FS i) r) as [[Hi' | Hi'] | Hi'].
+              { apply order_g_FS in Hi. rewrite Hi' in Hi. inv Hi. }
+              { contradiction. }
+              rewrite Hq. rewrite subtract_one_FS. reflexivity.
+            -- (* (p (p (i + 1))) - 1 > r *)
+              destruct (order_cases' (p (FS i)) r) as [[Hpi' | Hpi'] | Hpi'].
+              1, 3: rewrite Hpi' in Hpi; inv Hpi. clear Hpi'.
+              destruct (order_cases' (FS i) r) as [[Hi' | Hi'] | Hi'].
+              { apply order_g_FS in Hi. rewrite Hi' in Hi. inv Hi. }
+              { contradiction. }
+              rewrite Hq. rewrite subtract_one_FS. reflexivity.
+        + (* p (i + 1) > r *)
+          rewrite Hp. specialize (Hq (p' i)). rewrite Hp in Hq.
+          rewrite FS_subtract_one in Hq. rewrite Hqp in Hq.
+          destruct (order_cases' (subtract_one (p (FS i)) r Hpi) r) as
+            [[Hpis | Hpis] | Hpis].
+          * (* (p (i + 1)) - 1 < r *)
+            (* contradiction *)
+            apply subtract_one_l in Hpis.
+            destruct Hpis as [Hpis | Hpis]; rewrite Hpi in Hpis; inv Hpis.
+          * (* (p (i + 1)) - 1 = r *)
+            destruct (order_cases' (FS i) r) as [[Hi' | Hi'] | Hi'].
+            1, 2: apply order_g_FS in Hi; rewrite Hi' in Hi; inv Hi.
+            rewrite Hq. rewrite subtract_one_FS. reflexivity.
+          * (* (p (i + 1)) - 1 > r *)
+            destruct (order_cases' (FS i) r) as [[Hi' | Hi'] | Hi'].
+            1, 2: apply order_g_FS in Hi; rewrite Hi' in Hi; inv Hi.
+            rewrite Hq. rewrite subtract_one_FS. reflexivity.
+    }
+  Qed.
+
+  Ltac cases a b name := destruct (order_cases' a b) as [[name | name] | name].
+
+
+  (* TODO: fix so its remove (p r) for q. How was this true for the prev defn???
+   I thikn it's because removing at i means that anything going to i before goes to
+   p i now, which is basically equivalent? i and p i are "next" to each other so it
+   was also correct. *)
+  Lemma remove_at_permutation_correct' {n} (p q : fin (S (S n)) -> fin (S (S n))) r
+        (Hpq : forall i, p (q i) = i)
+        (Hqp : forall i, q (p i) = i) :
+    let p' := projT1 (remove_at_permutation p r (bijective_injective _ _ Hqp)) in
+    let q' := projT1 (remove_at_permutation q (p r) (bijective_injective _ _ Hpq)) in
+    (forall i, p' (q' i) = i).
+  Proof.
+    destruct (remove_at_permutation p r _) as (p' & Hp).
+    destruct (remove_at_permutation q (p r) _) as (q' & Hq).
+    cbn in *. intro i.
+    specialize (Hq i).
+    cases i (p r) Hi.
+    - (* i < p r *)
+      cases (q (fin_S i)) (p r) Hqi.
+      + (* q i < p r *)
+        rewrite Hq. specialize (Hp (q' i)). rewrite Hq in Hp.
+        rewrite fin_S_not_highest in Hp. rewrite Hpq in Hp.
+        cases (not_highest (q (fin_S i)) (p r) Hqi) r Hqi'.
+        * (* q i < r *)
+          cases (fin_S i) r Hi'.
+          -- (* i < r *)
+            rewrite Hp. rewrite not_highest_fin_S. reflexivity.
+          -- (* i = r *)
+            cases (p (fin_S i)) r Hpi; try contradiction.
+            ++ (* p i < r *)
+              (* contradiction: i < p i < i *)
+              admit.
+            ++ (* p i > r *)
+              (* p i > i > q i*)
+              rewrite Hp.
+  Admitted.
+
+  Lemma remove_at_permutation_vectors {n} (v1 v2 : vec (S (S n))) i p q Hp Hq p' q'
+        (Hp' : p' = projT1 (remove_at_permutation p i Hp))
+        (Hq' : q' = projT1 (remove_at_permutation q (p i) Hq))
+        (Hpq : forall i, p (q i) = i)
+        (Hqp : forall i, q (p i) = i)
+        (Hpq' : forall i, p' (q' i) = i)
+        (Hqp' : forall i, q' (p' i) = i)
+        (Hsb1 : forall i, v1 i ~ v2 (p i))
+        (Hsb2 : forall i, v2 i ~ v1 (q i)) :
+    forall j : fin (S n),
+      remove_vec v1 i j ~
+      remove_vec v2 (p i) (p' j).
+  Proof.
+    intros. subst. destruct (remove_at_permutation p) as (p' & Hp'). cbn in *.
+    destruct (remove_at_permutation q) as (q' & Hq'). cbn in *.
+    specialize (Hp' j).
+    cases j i Hj.
+    - (* j < i *)
+      rewrite <- remove_vec_index_before'; auto.
+      cases (p (fin_S j)) i Hpj.
+      + (* p j < i *)
+        cases (p' j) (p i) Hpjpi.
+        * (* p j < p i *)
+          rewrite <- remove_vec_index_before'; auto.
+          rewrite Hp'. rewrite fin_S_not_highest. apply Hsb1.
+        * (* p j = p i, contradiction since j < i *)
+          rewrite Hp' in Hpjpi. rewrite <- order_not_highest_equal in Hpjpi.
+          apply order_eq in Hpjpi. apply Hp in Hpjpi. subst.
+          rewrite order_fin_S_equal in Hj. inv Hj.
+        * (* p j > p i *)
+          (* (so p i < p j < i) *)
+          rewrite <- remove_vec_index_after'; auto. rewrite Hp'.
+          apply (f_equal q') in Hp'. rewrite Hqp' in Hp'.
+          (*
+          rewrite Hp' at 2. rewrite Hpq'.
+          specialize (Hq' (not_highest (p (fin_S j)) i Hpj)).
+          rewrite fin_S_not_highest in Hq'. rewrite Hqp in Hq'.
+          cases (not_highest (p (fin_S j)) i Hpj) (p i) Hpjpi'.
+          1, 2: rewrite Hp', Hpq' in Hpjpi; rewrite Hpjpi in Hpjpi'; inv Hpjpi'.
+          cases (q (FS (not_highest (p (fin_S j)) i Hpj))) (p i) Hqpj.
+          -- (* q (p j + 1) < p i *)
+            rewrite Hp' at 1. rewrite Hq'. rewrite fin_S_not_highest.
+            symmetry. apply Hsb2.
+          -- (* q (p j + 1) = p i *)
+            (* so p j + 1 = p (p i) *)
+            apply order_eq in Hqpj. apply (f_equal p) in Hqpj. rewrite Hpq in Hqpj.
+            rewrite Hqpj in Hq'. do 2 rewrite Hqp in Hq'.
+            cases i (p i) Hi; try contradiction.
+            ++ admit. (* contradiction *)
+            ++ rewrite Hq' in Hp'.
+               clear Hpjpi.
+               clear Hpjpi'.
+               clear Hqpj. clear Hq'.
+               revert Hpj. rewrite Hp'. intros. rewrite Hq'.
+              (* q (q (p j + 1)) < p i *)
+              (* so q (q (p (p i))) = i < p i, contradiction *)
+              rewrite Hp' at 1. rewrite Hq'. rewrite Hqp'. rewrite fin_S_not_highest.
+
+            symmetry. apply Hsb2.
+          --
+          destruct (order_cases' (fin_S j) i) as [[Hj' | Hj'] | Hj'].
+          2, 3: rewrite order_fin_S in Hj; rewrite Hj' in Hj; inv Hj.
+          rewrite Hq' in Hp'.
+          rewrite Hp' at 1. rewrite fin_S_not_highest. rewrite Hq'.
+          revert Hpj. rewrite Hp' in *. rewrite Hp'.
+
+      + apply order_eq in Hpj. rewrite Hpj in Hp'.
+        destruct (order_cases' (p i) i) as [[Hpi | Hpi] | Hpi]; try contradiction.
+        * rewrite Hp' in *. rewrite <- order_not_highest_equal in Hp'j.
+          rewrite order_reflexive in Hp'j. inv Hp'j.
+        * apply (f_equal q') in Hp'. rewrite Hqp' in Hp'.
+          rewrite Hp' in *. rewrite Hpq' in *.
+          specialize (Hq' (subtract_one (p i) i Hpi)).
+      + apply (f_equal q') in Hp'. rewrite Hqp' in Hp'.
+        rewrite Hp' in *. rewrite Hpq' in *.
+          specialize (Hq' (subtract_one (p i) i Hpi)). admit.
+      +
+  Qed.
+           *)
+  Abort.
+
+  Lemma schedule_permutation n (v1 v2 : vec n) i (p q : fin n -> fin n)
+        (Hbound1 : forall i, choiceI_bound 1 (v1 i))
+        (Hbound2 : forall i, choiceI_bound 1 (v2 i))
+        (Hpq : forall i, p (q i) = i)
+        (Hqp : forall i, q (p i) = i)
+        (Hsb1 : forall i, v1 i ~ v2 (p i))
+        (Hsb2 : forall i, v2 i ~ v1 (q i)) :
+    schedule n v1 (Some i) ~ schedule n v2 (Some (p i)).
+  Proof.
+    revert n v1 v2 i p q Hbound1 Hbound2 Hpq Hqp Hsb1 Hsb2.
+    coinduction r CIH.
+    symmetric using idtac.
+    {
+      intros. rewrite <- (Hqp i) at 2.
+      eapply H; auto.
+    }
+    intros n v1 v2 i p q Hbound1 Hbound2 Hpq Hqp Hsb1 Hsb2 l t Ht. cbn in *.
+    destruct l.
+    - apply trans_schedule_thread_tau_some in Ht; auto.
+      decompose [or] Ht; clear Ht.
+      + (* thread is finished *)
+        destruct H as (n' & i' & Ht & ? & Hequ). subst.
+        pose proof (Hsb1 i). step in H. destruct H as [Hf _].
+        edestruct Hf as [? ? ?]; eauto.
+        eapply trans_thread_schedule_val_SS in H.
+        eexists. apply H. rewrite Hequ.
+        pose proof (@remove_at_permutation_correct _ _ _ i Hpq Hqp) as (Hpq' & Hqp').
+        eapply CIH; clear CIH; cbn; try solve [apply remove_vec_choiceI_bound; auto].
+        apply Hpq'. apply Hqp'.
+        * admit. (* eapply remove_at_permutation_vectors; eauto. *)
+        * admit. (* intros. destruct (remove_at_permutation q) as (q' & Hq'). cbn in *. *)
+      + (* tau step *)
+        destruct n; try inv i.
+        destruct H0 as (t' & Ht & Hbound & Hequ).
+        pose proof (Hsb1 i). step in H. destruct H as [Hf _].
+        edestruct Hf as [? ? ?]; eauto.
+        pose proof (trans_choiceI_bound _ _ _ _ _ (Hbound2 _) H) as Hbound'.
+        apply trans_thread_schedule_tau in H.
+        eexists; eauto. rewrite Hequ.
+        eapply CIH; clear CIH; eauto; try solve [apply replace_vec_choiceI_bound; auto].
+        * intros. destruct (Fin.eq_dec i i0).
+          -- subst. do 2 (rewrite replace_vec_eq; auto).
+          -- do 2 (rewrite replace_vec_neq; auto). intro.
+             apply (f_equal q) in H1. do 2 rewrite Hqp in H1. contradiction.
+        * intros. destruct (Fin.eq_dec (p i) i0).
+          -- subst. rewrite Hqp. do 2 (rewrite replace_vec_eq; auto). symmetry; auto.
+          -- do 2 (rewrite replace_vec_neq; auto). intro.
+             apply (f_equal p) in H1. rewrite Hpq in H1. contradiction.
+      + (* The thread yields *)
+        destruct n; try inv i.
+        destruct H as (k & Hvis & i' & Hequ).
+        pose proof Hvis as Hvis'.
+        eapply sbisim_visible in Hvis'. 5: apply Hsb1. all: auto.
+        destruct Hvis' as (k' & Hvis' & Hk).
+        exists (schedule (S n) (replace_vec v2 (p i) (k' tt)) (Some (p i'))).
+        2: { rewrite Hequ.
+             eapply CIH; clear CIH; eauto.
+             - intro. apply replace_vec_choiceI_bound; auto.
+               eapply visible_choiceI_bound in Hvis; eauto.
+               eapply trans_choiceI_bound; eauto. constructor. reflexivity.
+             - intro. apply replace_vec_choiceI_bound; auto.
+               eapply visible_choiceI_bound in Hvis'; eauto.
+               eapply trans_choiceI_bound; eauto. constructor. reflexivity.
+             - intros. destruct (Fin.eq_dec i i0).
+               + subst. do 2 rewrite replace_vec_eq; auto.
+               + do 2 (rewrite replace_vec_neq; auto). intro.
+                 apply (f_equal q) in H. do 2 rewrite Hqp in H. contradiction.
+             - intros. destruct (Fin.eq_dec (p i) i0).
+               + subst. rewrite Hqp. do 2 rewrite replace_vec_eq; auto. symmetry; auto.
+               + do 2 (rewrite replace_vec_neq; auto). intro.
+                 apply (f_equal p) in H. rewrite Hpq in H. contradiction.
+        }
+        apply visible_yield_trans_schedule; auto.
+      + (* the thread spawns a new thread *)
+        destruct H as (k & Hvis & Hequ).
+        destruct n; try inv i.
+        pose proof Hvis as Hvis'.
+        eapply sbisim_visible in Hvis'. 5: apply Hsb1. all: eauto.
+        2: { constructor. apply true. }
+        destruct Hvis' as (k' & Hvis' & ?).
+        pose proof (cons_permutation_correct _ _ Hpq Hqp).
+        destruct (cons_permutation p) as (p' & Hp1 & Hp2).
+        destruct (cons_permutation q) as (q' & Hq1 & Hq2). cbn in *.
+        destruct H0 as (Hpq' & Hqp').
+        exists (schedule (S (S n))
+                    (cons_vec (k' true)
+                              (replace_vec v2 (p i) (k' false)))
+                    (Some (p' (FS i)))).
+        2: {
+          assert (Hbound: forall b, choiceI_bound 1 (k b)). {
+            intros. eapply visible_choiceI_bound in Hvis; eauto.
+            eapply trans_choiceI_bound; eauto. constructor. reflexivity.
+          }
+          assert (Hbound': forall b, choiceI_bound 1 (k' b)). {
+            intros. eapply visible_choiceI_bound in Hvis'; eauto.
+            eapply trans_choiceI_bound; eauto. constructor. reflexivity.
+          }
+          rewrite Hequ. eapply CIH; auto;
+            try solve [apply cons_vec_choiceI_bound; auto;
+                       apply replace_vec_choiceI_bound; auto].
+          - intros. dependent destruction i0.
+            + rewrite Hp1. cbn. auto.
+            + rewrite Hp2. cbn. destruct (Fin.eq_dec i i0).
+              * subst. do 2 (rewrite replace_vec_eq; auto).
+              * do 2 (rewrite replace_vec_neq; auto). intro.
+                apply (f_equal q) in H0. do 2 rewrite Hqp in H0. contradiction.
+          - intros. dependent destruction i0.
+            + rewrite Hq1. cbn. symmetry. auto.
+            + rewrite Hq2. cbn. destruct (Fin.eq_dec (p i) i0).
+              * subst. rewrite Hqp. do 2 (rewrite replace_vec_eq; auto). symmetry; auto.
+              * do 2 (rewrite replace_vec_neq; auto). intro.
+                apply (f_equal p) in H0. rewrite Hpq in H0. contradiction.
+        }
+        rewrite Hp2. apply visible_spawn_trans_schedule; auto.
+    - apply trans_schedule_obs in Ht.
+      destruct Ht as (k & i' & s & ? & ? & Hvis & Hequ). inv H. rename i' into i.
+      destruct n; try inv i.
+      pose proof Hvis as Hvis'.
+      eapply sbisim_visible in Hvis'. 5: apply Hsb1. all: eauto.
+      destruct Hvis' as (k' & Hvis' & ?).
+      exists (schedule (S n) (replace_vec v2 (p i) (k' v)) (Some (p i))).
+      2: {
+        assert (Hbound: forall x, choiceI_bound 1 (k x)). {
+          intros. eapply visible_choiceI_bound in Hvis; eauto.
+          eapply trans_choiceI_bound; eauto. constructor. reflexivity.
+        }
+        assert (Hbound': forall x, choiceI_bound 1 (k' x)). {
+          intros. eapply visible_choiceI_bound in Hvis'; eauto.
+          eapply trans_choiceI_bound; eauto. constructor. reflexivity.
+        }
+        rewrite Hequ. eapply CIH; clear CIH; eauto;
+          try solve [apply replace_vec_choiceI_bound; auto].
+        - intros. destruct (Fin.eq_dec i i0).
+          + subst. do 2 rewrite replace_vec_eq; auto.
+          + do 2 (rewrite replace_vec_neq; auto). intro.
+            apply (f_equal q) in H0. do 2 rewrite Hqp in H0. contradiction.
+        - intros. destruct (Fin.eq_dec (p i) i0).
+          + subst. rewrite Hqp. do 2 rewrite replace_vec_eq; auto. symmetry; auto.
+          + do 2 (rewrite replace_vec_neq; auto). intro.
+            apply (f_equal p) in H0. rewrite Hpq in H0. contradiction.
+      }
+      apply visible_stateE_trans_schedule; auto.
+    - pose proof (trans_schedule_val_1 _ _ _ _ _ Ht). subst.
+      pose proof (trans_val_inv Ht).
+      pose proof (Hsb1 i). step in H0. destruct H0 as [Hf _].
+      pose proof (trans_schedule_thread_val _ _ _ _ Ht) as Hv1.
+      edestruct Hf; eauto.
+      apply trans_thread_schedule_val_1 in H0. eexists; eauto. rewrite H. reflexivity.
+  Abort.
+
+  (*
+  Lemma schedule_perm_2 n (v1 v2 : vec n) i1 i2
+        (Hbound1 : forall i, choiceI_bound 1 (v1 i))
+        (Hbound2 : forall i, choiceI_bound 1 (v2 i)) :
+    (i1 = i2 /\ forall i, v1 i ~ v2 i) \/
+      (i1 = i2 /\
+         exists i3 i4,
+           i3 <> i4 /\
+             i1 <> i3 /\
+             i1 <> i4 /\
+             v1 i3 ~ v2 i4 /\
+             v2 i3 ~ v1 i4 /\
+             (forall i, i <> i3 -> i <> i4 -> v1 i ~ v2 i)) \/
+      (i1 <> i2 /\
+         v1 i1 ~ v2 i2 /\
+         v2 i1 ~ v1 i2 /\
+         (forall i, i <> i1 -> i <> i2 -> v1 i ~ v2 i)) ->
+    schedule n v1 (Some i1) ~ schedule n v2 (Some i2).
+  Proof.
+    revert n v1 v2 i1 i2 Hbound1 Hbound2.
+    coinduction r CIH.
+    symmetric using idtac.
+    {
+      intros. apply H; auto. decompose [or] H0; clear H0.
+      - left. destruct H1. split; auto. symmetry. auto.
+      - right. left. destruct H2 as (? & i3 & i4 & ? & ? & ? & ? & ? & ?). subst.
+        split; auto. exists i4, i3. split; [| split; [| split]]; auto.
+        split; [| split]; symmetry; auto.
+      - right. right. destruct H2 as (? & ? & ? & ?).
+        split; auto. split; [| split]; symmetry; auto.
+    }
+    intros n v1 v2 i1 i2 Hbound1 Hbound2 Hi l t Ht. cbn in *.
+    destruct l.
+    - apply trans_schedule_thread_tau_some in Ht; auto.
+      decompose [or] Ht; clear Ht.
+      + (* thread is finished *)
+        destruct H as (n' & i & Ht & ? & Hequ). subst.
+        destruct Hi as [
+            (? & Hv) | [
+              (? & i3 & i4 & Hneq1 & Hneq2 & Hneq3 & Hi1sb & Hi2sb & Hothers) |
+              (Hneq & Hi1sb & Hi2sb & Hothers)]].
+        * (* no swapped elements *)
+          subst. pose proof (Hv i2). step in H. destruct H as [Hf _].
+          edestruct Hf as [? ? ?]; eauto.
+          eapply trans_thread_schedule_val_SS in H.
+          eexists. apply H. rewrite Hequ. apply CIH; cbn.
+          admit. admit.
+          left. split; eauto.
+          intros. apply remove_vec_vec_relation; auto.
+        * (* swapped elements are elsewhere in v: i3 and i4 *)
+          subst. pose proof (Hothers i2 Hneq2 Hneq3).
+          step in H. destruct H as [Hf _].
+          edestruct Hf as [? ? ?]; eauto.
+          rewrite <- (of_nat_to_nat_inv i) in Hequ. rewrite <- (of_nat_to_nat_inv i2) in Hequ.
+          destruct (to_nat i) as [i' Hi'] eqn:Hi.
+          destruct (to_nat i2) as [i2' Hi2'] eqn:Hi2. cbn in Hequ.
+          destruct (to_nat i3) as [i3' Hi3'] eqn:Hi3.
+          destruct (to_nat i4) as [i4' Hi4'] eqn:Hi4.
+          assert (i3' < i2' \/ i3' > i2').
+          {
+            rewrite <- (of_nat_to_nat_inv i3) in Hneq2. rewrite Hi3 in Hneq2.
+            rewrite <- (of_nat_to_nat_inv i2) in Hneq2. rewrite Hi2 in Hneq2. cbn in Hneq2.
+            rewrite <- of_nat_lt_sig1_neq in Hneq2. lia.
+          }
+          assert (i4' < i2' \/ i4' > i2').
+          {
+            rewrite <- (of_nat_to_nat_inv i4) in Hneq3. rewrite Hi4 in Hneq3.
+            rewrite <- (of_nat_to_nat_inv i2) in Hneq3. rewrite Hi2 in Hneq3. cbn in Hneq3.
+            rewrite <- of_nat_lt_sig1_neq in Hneq3. lia.
+          }
+          destruct H1, H2.
+          (* TODO: clean up all this copy and paste *)
+          (* i3' < i2', i4' < i2' *)
+          {
+            assert (Hneq4: i3' <> i4').
+            {
+              rewrite of_nat_lt_sig1_neq.
+              rewrite <- (of_nat_to_nat_inv i3) in Hneq1. rewrite Hi3 in Hneq1.
+              rewrite <- (of_nat_to_nat_inv i4) in Hneq1. rewrite Hi4 in Hneq1.
+              apply Hneq1.
+            }
+            destruct (PeanoNat.Nat.eq_dec i' i3'); [| destruct (PeanoNat.Nat.eq_dec i' i4')].
+            {
+              (* we are going to i3' next *)
+              subst. rename Hi' into Hi3''.
+              assert (Hi4'' : i4' < S n') by lia.
+              apply trans_thread_schedule_val_SS with (i':=(of_nat_lt Hi4'')) in H.
+              eexists. apply H. rewrite Hequ. apply CIH; clear CIH. admit. admit.
+              right. right. split.
+              {
+                intro. eapply f_equal in H3. do 2 rewrite to_nat_of_nat in H3.
+                inv H3. contradiction.
+              }
+              split; [| split].
+              - rewrite <- (of_nat_to_nat_inv i2). rewrite Hi2. cbn.
+                do 2 (erewrite <- remove_vec_index_before; eauto).
+                rewrite <- (of_nat_to_nat_inv i3) in Hi1sb.
+                rewrite <- (of_nat_to_nat_inv i4) in Hi1sb.
+                rewrite Hi3, Hi4 in Hi1sb. cbn in Hi1sb.
+                apply Hi1sb.
+              - rewrite <- (of_nat_to_nat_inv i2). rewrite Hi2. cbn.
+                do 2 (erewrite <- remove_vec_index_before; eauto).
+                rewrite <- (of_nat_to_nat_inv i3) in Hi2sb.
+                rewrite <- (of_nat_to_nat_inv i4) in Hi2sb.
+                rewrite Hi3, Hi4 in Hi2sb. cbn in Hi2sb.
+                apply Hi2sb.
+              - intros.
+                destruct (to_nat i0) as [i0' Hi0'] eqn:Hi0.
+                rewrite <- (of_nat_to_nat_inv i2). rewrite Hi2.
+                rewrite <- (of_nat_to_nat_inv i0). rewrite Hi0. cbn.
+                rewrite <- (of_nat_to_nat_inv i0) in H3, H4. rewrite Hi0 in H3, H4. cbn in *.
+                assert (i0' < i2' \/ i0' = i2' \/ i0' > i2') by lia.
+                destruct H5 as [? | [? | ?]].
+                + assert (Hi0'' : i0' < S (S n')) by lia.
+                  specialize (Hothers (of_nat_lt Hi0'')).
+                  rewrite <- of_nat_lt_sig1_neq in H3.
+                  rewrite <- of_nat_lt_sig1_neq in H4.
+                  do 2 (erewrite <- remove_vec_index_before; eauto).
+                  eapply Hothers; eauto.
+                  * rewrite <- (of_nat_to_nat_inv i3). rewrite Hi3. cbn.
+                    rewrite <- of_nat_lt_sig1_neq. auto.
+                  * rewrite <- (of_nat_to_nat_inv i4). rewrite Hi4. cbn.
+                    rewrite <- of_nat_lt_sig1_neq. auto.
+                + subst. rename i2' into i0'.
+                  assert (Hi0'' : S i0' < S (S n')) by lia.
+                  specialize (Hothers (of_nat_lt Hi0'')).
+                  do 2 (erewrite <- remove_vec_index_eq; eauto).
+                  eapply Hothers; eauto.
+                  * rewrite <- (of_nat_to_nat_inv i3). rewrite Hi3.
+                    rewrite <- of_nat_lt_sig1_neq. cbn. lia.
+                  * rewrite <- (of_nat_to_nat_inv i4). rewrite Hi4.
+                    rewrite <- of_nat_lt_sig1_neq. cbn. lia.
+                + assert (Hi0'' : S i0' < S (S n')) by lia.
+                  specialize (Hothers (of_nat_lt Hi0'')).
+                  do 2 (erewrite <- remove_vec_index_after; eauto).
+                  eapply Hothers; eauto.
+                  * rewrite <- (of_nat_to_nat_inv i3). rewrite Hi3.
+                    rewrite <- of_nat_lt_sig1_neq. cbn. lia.
+                  * rewrite <- (of_nat_to_nat_inv i4). rewrite Hi4.
+                    rewrite <- of_nat_lt_sig1_neq. cbn. lia.
+            }
+            {
+              (* we are going to i4' next *)
+              subst. rename Hi' into Hi4''.
+              assert (Hi3'' : i3' < S n') by lia.
+              apply trans_thread_schedule_val_SS with (i':=(of_nat_lt Hi3'')) in H.
+              eexists. apply H. rewrite Hequ. apply CIH; clear CIH. admit. admit.
+              right. right. split.
+              {
+                intro. eapply f_equal in H3. do 2 rewrite to_nat_of_nat in H3.
+                inv H3. contradiction.
+              }
+              split; [| split].
+              - rewrite <- (of_nat_to_nat_inv i2). rewrite Hi2. cbn.
+                do 2 (erewrite <- remove_vec_index_before; eauto).
+                rewrite <- (of_nat_to_nat_inv i3) in Hi2sb.
+                rewrite <- (of_nat_to_nat_inv i4) in Hi2sb.
+                rewrite Hi3, Hi4 in Hi2sb. cbn in Hi2sb.
+                symmetry. apply Hi2sb.
+              - rewrite <- (of_nat_to_nat_inv i2). rewrite Hi2. cbn.
+                do 2 (erewrite <- remove_vec_index_before; eauto).
+                rewrite <- (of_nat_to_nat_inv i3) in Hi1sb.
+                rewrite <- (of_nat_to_nat_inv i4) in Hi1sb.
+                rewrite Hi3, Hi4 in Hi1sb. cbn in Hi1sb.
+                symmetry. apply Hi1sb.
+              - intros.
+                destruct (to_nat i0) as [i0' Hi0'] eqn:Hi0.
+                rewrite <- (of_nat_to_nat_inv i2). rewrite Hi2.
+                rewrite <- (of_nat_to_nat_inv i0). rewrite Hi0. cbn.
+                rewrite <- (of_nat_to_nat_inv i0) in H3, H4. rewrite Hi0 in H3, H4. cbn in *.
+                assert (i0' < i2' \/ i0' = i2' \/ i0' > i2') by lia.
+                destruct H5 as [? | [? | ?]].
+                + assert (Hi0'' : i0' < S (S n')) by lia.
+                  specialize (Hothers (of_nat_lt Hi0'')).
+                  rewrite <- of_nat_lt_sig1_neq in H3.
+                  rewrite <- of_nat_lt_sig1_neq in H4.
+                  do 2 (erewrite <- remove_vec_index_before; eauto).
+                  eapply Hothers; eauto.
+                  * rewrite <- (of_nat_to_nat_inv i3). rewrite Hi3. cbn.
+                    rewrite <- of_nat_lt_sig1_neq. auto.
+                  * rewrite <- (of_nat_to_nat_inv i4). rewrite Hi4. cbn.
+                    rewrite <- of_nat_lt_sig1_neq. auto.
+                + subst. rename i2' into i0'.
+                  assert (Hi0'' : S i0' < S (S n')) by lia.
+                  specialize (Hothers (of_nat_lt Hi0'')).
+                  do 2 (erewrite <- remove_vec_index_eq; eauto).
+                  eapply Hothers; eauto.
+                  * rewrite <- (of_nat_to_nat_inv i3). rewrite Hi3.
+                    rewrite <- of_nat_lt_sig1_neq. cbn. lia.
+                  * rewrite <- (of_nat_to_nat_inv i4). rewrite Hi4.
+                    rewrite <- of_nat_lt_sig1_neq. cbn. lia.
+                + assert (Hi0'' : S i0' < S (S n')) by lia.
+                  specialize (Hothers (of_nat_lt Hi0'')).
+                  do 2 (erewrite <- remove_vec_index_after; eauto).
+                  eapply Hothers; eauto.
+                  * rewrite <- (of_nat_to_nat_inv i3). rewrite Hi3.
+                    rewrite <- of_nat_lt_sig1_neq. cbn. lia.
+                  * rewrite <- (of_nat_to_nat_inv i4). rewrite Hi4.
+                    rewrite <- of_nat_lt_sig1_neq. cbn. lia.
+            }
+            {
+              (* we are going to i', which is not one of the swapped elements *)
+              assert (Hi3'' : i3' < S n') by lia.
+              assert (Hi4'' : i4' < S n') by lia.
+              apply trans_thread_schedule_val_SS with (i':=(of_nat_lt Hi')) in H.
+              eexists. apply H. rewrite Hequ. apply CIH; clear CIH. admit. admit.
+              right. left. split; auto.
+              exists (of_nat_lt Hi3''), (of_nat_lt Hi4'').
+              split; [| split; [| split]]; try solve [rewrite <- of_nat_lt_sig1_neq; auto].
+              split; [| split].
+              - rewrite <- (of_nat_to_nat_inv i2). rewrite Hi2. cbn.
+                do 2 (erewrite <- remove_vec_index_before; eauto).
+                rewrite <- (of_nat_to_nat_inv i3) in Hi1sb.
+                rewrite <- (of_nat_to_nat_inv i4) in Hi1sb.
+                rewrite Hi3, Hi4 in Hi1sb. cbn in Hi1sb.
+                apply Hi1sb.
+              - rewrite <- (of_nat_to_nat_inv i2). rewrite Hi2. cbn.
+                do 2 (erewrite <- remove_vec_index_before; eauto).
+                rewrite <- (of_nat_to_nat_inv i3) in Hi2sb.
+                rewrite <- (of_nat_to_nat_inv i4) in Hi2sb.
+                rewrite Hi3, Hi4 in Hi2sb. cbn in Hi2sb.
+                apply Hi2sb.
+              - intros.
+                destruct (to_nat i0) as [i0' Hi0'] eqn:Hi0.
+                rewrite <- (of_nat_to_nat_inv i2). rewrite Hi2.
+                rewrite <- (of_nat_to_nat_inv i0). rewrite Hi0. cbn.
+                rewrite <- (of_nat_to_nat_inv i0) in H3, H4. rewrite Hi0 in H3, H4. cbn in *.
+                assert (i0' < i2' \/ i0' = i2' \/ i0' > i2') by lia.
+                destruct H5 as [? | [? | ?]].
+                + assert (Hi0'' : i0' < S (S n')) by lia.
+                  specialize (Hothers (of_nat_lt Hi0'')).
+                  rewrite <- of_nat_lt_sig1_neq in H3.
+                  rewrite <- of_nat_lt_sig1_neq in H4.
+                  do 2 (erewrite <- remove_vec_index_before; eauto).
+                  eapply Hothers; eauto.
+                  * rewrite <- (of_nat_to_nat_inv i3). rewrite Hi3. cbn.
+                    rewrite <- of_nat_lt_sig1_neq. auto.
+                  * rewrite <- (of_nat_to_nat_inv i4). rewrite Hi4. cbn.
+                    rewrite <- of_nat_lt_sig1_neq. auto.
+                + subst. rename i2' into i0'.
+                  assert (Hi0'' : S i0' < S (S n')) by lia.
+                  specialize (Hothers (of_nat_lt Hi0'')).
+                  do 2 (erewrite <- remove_vec_index_eq; eauto).
+                  eapply Hothers; eauto.
+                  * rewrite <- (of_nat_to_nat_inv i3). rewrite Hi3.
+                    rewrite <- of_nat_lt_sig1_neq. cbn. lia.
+                  * rewrite <- (of_nat_to_nat_inv i4). rewrite Hi4.
+                    rewrite <- of_nat_lt_sig1_neq. cbn. lia.
+                + assert (Hi0'' : S i0' < S (S n')) by lia.
+                  specialize (Hothers (of_nat_lt Hi0'')).
+                  do 2 (erewrite <- remove_vec_index_after; eauto).
+                  eapply Hothers; eauto.
+                  * rewrite <- (of_nat_to_nat_inv i3). rewrite Hi3.
+                    rewrite <- of_nat_lt_sig1_neq. cbn. lia.
+                  * rewrite <- (of_nat_to_nat_inv i4). rewrite Hi4.
+                    rewrite <- of_nat_lt_sig1_neq. cbn. lia.
+            }
+          }
+          (* i3' < i2', i4' > i2' *)
+          {
+            destruct i4'. inv H2.
+            assert (Hneq4: i3' <> i4').
+            {
+              rewrite <- (of_nat_to_nat_inv i3) in Hneq1. rewrite Hi3 in Hneq1.
+              rewrite <- (of_nat_to_nat_inv i4) in Hneq1. rewrite Hi4 in Hneq1.
+              rewrite <- of_nat_lt_sig1_neq in Hneq1. cbn in Hneq1. lia.
+            }
+
+            destruct (PeanoNat.Nat.eq_dec i' i3'); [| destruct (PeanoNat.Nat.eq_dec i' i4')].
+            {
+              (* we are going to i3' next *)
+              subst. rename Hi' into Hi3''.
+              (* destruct i4'. inv H2. (* subtract i4' by one *) *)
+              assert (Hi4'' : i4' < S n') by lia.
+              apply trans_thread_schedule_val_SS with (i':=(of_nat_lt Hi4'')) in H.
+              eexists. apply H. rewrite Hequ. apply CIH; clear CIH. admit. admit.
+              right. right. split.
+              {
+                intro. eapply f_equal in H3. do 2 rewrite to_nat_of_nat in H3.
+                inv H3. contradiction.
+              }
+              split; [| split].
+              - rewrite <- (of_nat_to_nat_inv i2). rewrite Hi2. cbn.
+                erewrite <- remove_vec_index_before; eauto.
+                assert (i4' = i2' \/ i4' > i2') by lia. destruct H3.
+                + subst. erewrite <- remove_vec_index_eq; eauto.
+                  rewrite <- (of_nat_to_nat_inv i3) in Hi1sb.
+                  rewrite <- (of_nat_to_nat_inv i4) in Hi1sb.
+                  rewrite Hi3, Hi4 in Hi1sb. cbn in Hi1sb.
+                  apply Hi1sb.
+                + erewrite <- remove_vec_index_after; eauto.
+                  rewrite <- (of_nat_to_nat_inv i3) in Hi1sb.
+                  rewrite <- (of_nat_to_nat_inv i4) in Hi1sb.
+                  rewrite Hi3, Hi4 in Hi1sb. cbn in Hi1sb.
+                  apply Hi1sb.
+              - rewrite <- (of_nat_to_nat_inv i2). rewrite Hi2. cbn.
+                erewrite <- remove_vec_index_before; eauto.
+                assert (i4' = i2' \/ i4' > i2') by lia. destruct H3.
+                + subst. erewrite <- remove_vec_index_eq; eauto.
+                  rewrite <- (of_nat_to_nat_inv i3) in Hi2sb.
+                  rewrite <- (of_nat_to_nat_inv i4) in Hi2sb.
+                  rewrite Hi3, Hi4 in Hi2sb. cbn in Hi2sb.
+                  apply Hi2sb.
+                + erewrite <- remove_vec_index_after; eauto.
+                  rewrite <- (of_nat_to_nat_inv i3) in Hi2sb.
+                  rewrite <- (of_nat_to_nat_inv i4) in Hi2sb.
+                  rewrite Hi3, Hi4 in Hi2sb. cbn in Hi2sb.
+                  apply Hi2sb.
+              - intros.
+                destruct (to_nat i0) as [i0' Hi0'] eqn:Hi0.
+                rewrite <- (of_nat_to_nat_inv i2). rewrite Hi2.
+                rewrite <- (of_nat_to_nat_inv i0). rewrite Hi0. cbn.
+                rewrite <- (of_nat_to_nat_inv i0) in H3, H4. rewrite Hi0 in H3, H4. cbn in *.
+                assert (i0' < i2' \/ i0' = i2' \/ i0' > i2') by lia.
+                destruct H5 as [? | [? | ?]].
+                + assert (Hi0'' : i0' < S (S n')) by lia.
+                  specialize (Hothers (of_nat_lt Hi0'')).
+                  rewrite <- of_nat_lt_sig1_neq in H3.
+                  rewrite <- of_nat_lt_sig1_neq in H4.
+                  do 2 (erewrite <- remove_vec_index_before; eauto).
+                  eapply Hothers; eauto.
+                  * rewrite <- (of_nat_to_nat_inv i3). rewrite Hi3. cbn.
+                    rewrite <- of_nat_lt_sig1_neq. auto.
+                  * rewrite <- (of_nat_to_nat_inv i4). rewrite Hi4.
+                    rewrite <- of_nat_lt_sig1_neq. cbn. lia.
+                + subst. rename i2' into i0'.
+                  assert (Hi0'' : S i0' < S (S n')) by lia.
+                  specialize (Hothers (of_nat_lt Hi0'')).
+                  do 2 (erewrite <- remove_vec_index_eq; eauto).
+                  eapply Hothers; eauto.
+                  * rewrite <- (of_nat_to_nat_inv i3). rewrite Hi3.
+                    rewrite <- of_nat_lt_sig1_neq. cbn. lia.
+                  * rewrite <- (of_nat_to_nat_inv i4). rewrite Hi4.
+                    rewrite <- of_nat_lt_sig1_neq in H4.
+                    rewrite <- of_nat_lt_sig1_neq. cbn. lia.
+                + assert (Hi0'' : S i0' < S (S n')) by lia.
+                  specialize (Hothers (of_nat_lt Hi0'')).
+                  do 2 (erewrite <- remove_vec_index_after; eauto).
+                  eapply Hothers; eauto.
+                  * rewrite <- (of_nat_to_nat_inv i3). rewrite Hi3.
+                    rewrite <- of_nat_lt_sig1_neq. cbn. lia.
+                  * rewrite <- (of_nat_to_nat_inv i4). rewrite Hi4.
+                    rewrite <- of_nat_lt_sig1_neq in H4.
+                    rewrite <- of_nat_lt_sig1_neq. cbn. lia.
+            }
+            {
+              (* we are going to i4' next *)
+              subst. rename Hi' into Hi4''.
+              assert (Hi3'' : i3' < S n') by lia.
+              apply trans_thread_schedule_val_SS with (i':=(of_nat_lt Hi3'')) in H.
+              eexists. apply H. rewrite Hequ. apply CIH; clear CIH. admit. admit.
+              right. right. split.
+              {
+                intro. eapply f_equal in H3. do 2 rewrite to_nat_of_nat in H3.
+                inv H3. contradiction.
+              }
+              split; [| split].
+              - rewrite <- (of_nat_to_nat_inv i2). rewrite Hi2.
+                assert (i4' = i2' \/ i4' > i2') by lia. destruct H3.
+                + subst. erewrite <- remove_vec_index_eq; eauto.
+                  erewrite <- remove_vec_index_before; eauto.
+                  rewrite <- (of_nat_to_nat_inv i3) in Hi2sb.
+                  rewrite <- (of_nat_to_nat_inv i4) in Hi2sb.
+                  rewrite Hi3, Hi4 in Hi2sb. cbn in Hi2sb.
+                  symmetry. eapply Hi2sb.
+                + erewrite <- remove_vec_index_after; eauto.
+                  erewrite <- remove_vec_index_before; eauto.
+                  rewrite <- (of_nat_to_nat_inv i3) in Hi2sb.
+                  rewrite <- (of_nat_to_nat_inv i4) in Hi2sb.
+                  rewrite Hi3, Hi4 in Hi2sb. cbn in Hi2sb.
+                  symmetry. apply Hi2sb.
+              - rewrite <- (of_nat_to_nat_inv i2). rewrite Hi2. cbn.
+                assert (i4' = i2' \/ i4' > i2') by lia. destruct H3.
+                + subst. erewrite <- remove_vec_index_eq; eauto.
+                  erewrite <- remove_vec_index_before; eauto.
+                  rewrite <- (of_nat_to_nat_inv i3) in Hi1sb.
+                  rewrite <- (of_nat_to_nat_inv i4) in Hi1sb.
+                  rewrite Hi3, Hi4 in Hi1sb. cbn in Hi1sb.
+                  symmetry. eapply Hi1sb.
+                + erewrite <- remove_vec_index_after; eauto.
+                  erewrite <- remove_vec_index_before; eauto.
+                  rewrite <- (of_nat_to_nat_inv i3) in Hi1sb.
+                  rewrite <- (of_nat_to_nat_inv i4) in Hi1sb.
+                  rewrite Hi3, Hi4 in Hi1sb. cbn in Hi1sb.
+                  symmetry. eapply Hi1sb.
+              - intros.
+                destruct (to_nat i0) as [i0' Hi0'] eqn:Hi0.
+                rewrite <- (of_nat_to_nat_inv i2). rewrite Hi2.
+                rewrite <- (of_nat_to_nat_inv i0). rewrite Hi0. cbn.
+                rewrite <- (of_nat_to_nat_inv i0) in H3, H4. rewrite Hi0 in H3, H4. cbn in *.
+                assert (i0' < i2' \/ i0' = i2' \/ i0' > i2') by lia.
+                destruct H5 as [? | [? | ?]].
+                + assert (Hi0'' : i0' < S (S n')) by lia.
+                  specialize (Hothers (of_nat_lt Hi0'')).
+                  rewrite <- of_nat_lt_sig1_neq in H3.
+                  rewrite <- of_nat_lt_sig1_neq in H4.
+                  do 2 (erewrite <- remove_vec_index_before; eauto).
+                  eapply Hothers; eauto.
+                  * rewrite <- (of_nat_to_nat_inv i3). rewrite Hi3. cbn.
+                    rewrite <- of_nat_lt_sig1_neq. auto.
+                  * rewrite <- (of_nat_to_nat_inv i4). rewrite Hi4.
+                    rewrite <- of_nat_lt_sig1_neq. cbn. lia.
+                + subst. rename i2' into i0'.
+                  assert (Hi0'' : S i0' < S (S n')) by lia.
+                  specialize (Hothers (of_nat_lt Hi0'')).
+                  do 2 (erewrite <- remove_vec_index_eq; eauto).
+                  eapply Hothers; eauto.
+                  * rewrite <- (of_nat_to_nat_inv i3). rewrite Hi3.
+                    rewrite <- of_nat_lt_sig1_neq. cbn. lia.
+                  * rewrite <- (of_nat_to_nat_inv i4). rewrite Hi4.
+                    rewrite <- of_nat_lt_sig1_neq in H3.
+                    rewrite <- of_nat_lt_sig1_neq. cbn. lia.
+                + assert (Hi0'' : S i0' < S (S n')) by lia.
+                  specialize (Hothers (of_nat_lt Hi0'')).
+                  do 2 (erewrite <- remove_vec_index_after; eauto).
+                  eapply Hothers; eauto.
+                  * rewrite <- (of_nat_to_nat_inv i3). rewrite Hi3.
+                    rewrite <- of_nat_lt_sig1_neq. cbn. lia.
+                  * rewrite <- (of_nat_to_nat_inv i4). rewrite Hi4.
+                    rewrite <- of_nat_lt_sig1_neq in H3.
+                    rewrite <- of_nat_lt_sig1_neq. cbn. lia.
+            }
+            {
+              (* we are going to i', which is not one of the swapped elements *)
+              assert (Hi3'' : i3' < S n') by lia.
+              assert (Hi4'' : i4' < S n') by lia.
+              apply trans_thread_schedule_val_SS with (i':=(of_nat_lt Hi')) in H.
+              eexists. apply H. rewrite Hequ. apply CIH; clear CIH. admit. admit.
+              right. left. split; auto.
+              exists (of_nat_lt Hi3''), (of_nat_lt Hi4'').
+              split; [| split; [| split]]; try solve [rewrite <- of_nat_lt_sig1_neq; auto].
+              split; [| split].
+              - rewrite <- (of_nat_to_nat_inv i2). rewrite Hi2. cbn.
+                erewrite <- remove_vec_index_before; eauto.
+                assert (i4' = i2' \/ i4' > i2') by lia. destruct H3.
+                + subst. erewrite <- remove_vec_index_eq; eauto.
+                  rewrite <- (of_nat_to_nat_inv i3) in Hi1sb.
+                  rewrite <- (of_nat_to_nat_inv i4) in Hi1sb.
+                  rewrite Hi3, Hi4 in Hi1sb. cbn in Hi1sb.
+                  apply Hi1sb.
+                + erewrite <- remove_vec_index_after; eauto.
+                  rewrite <- (of_nat_to_nat_inv i3) in Hi1sb.
+                  rewrite <- (of_nat_to_nat_inv i4) in Hi1sb.
+                  rewrite Hi3, Hi4 in Hi1sb. cbn in Hi1sb.
+                  apply Hi1sb.
+              - rewrite <- (of_nat_to_nat_inv i2). rewrite Hi2. cbn.
+                erewrite <- remove_vec_index_before; eauto.
+                assert (i4' = i2' \/ i4' > i2') by lia. destruct H3.
+                + subst. erewrite <- remove_vec_index_eq; eauto.
+                  rewrite <- (of_nat_to_nat_inv i3) in Hi2sb.
+                  rewrite <- (of_nat_to_nat_inv i4) in Hi2sb.
+                  rewrite Hi3, Hi4 in Hi2sb. cbn in Hi2sb.
+                  apply Hi2sb.
+                + subst. erewrite <- remove_vec_index_after; eauto.
+                  rewrite <- (of_nat_to_nat_inv i3) in Hi2sb.
+                  rewrite <- (of_nat_to_nat_inv i4) in Hi2sb.
+                  rewrite Hi3, Hi4 in Hi2sb. cbn in Hi2sb.
+                  apply Hi2sb.
+              - intros.
+                destruct (to_nat i0) as [i0' Hi0'] eqn:Hi0.
+                rewrite <- (of_nat_to_nat_inv i2). rewrite Hi2.
+                rewrite <- (of_nat_to_nat_inv i0). rewrite Hi0. cbn.
+                rewrite <- (of_nat_to_nat_inv i0) in H3, H4. rewrite Hi0 in H3, H4. cbn in *.
+                assert (i0' < i2' \/ i0' = i2' \/ i0' > i2') by lia.
+                destruct H5 as [? | [? | ?]].
+                + assert (Hi0'' : i0' < S (S n')) by lia.
+                  specialize (Hothers (of_nat_lt Hi0'')).
+                  rewrite <- of_nat_lt_sig1_neq in H3.
+                  rewrite <- of_nat_lt_sig1_neq in H4.
+                  do 2 (erewrite <- remove_vec_index_before; eauto).
+                  eapply Hothers; eauto.
+                  * rewrite <- (of_nat_to_nat_inv i3). rewrite Hi3. cbn.
+                    rewrite <- of_nat_lt_sig1_neq. auto.
+                  * rewrite <- (of_nat_to_nat_inv i4). rewrite Hi4.
+                    rewrite <- of_nat_lt_sig1_neq. cbn. lia.
+                + subst. rename i2' into i0'.
+                  assert (Hi0'' : S i0' < S (S n')) by lia.
+                  specialize (Hothers (of_nat_lt Hi0'')).
+                  do 2 (erewrite <- remove_vec_index_eq; eauto).
+                  eapply Hothers; eauto.
+                  * rewrite <- (of_nat_to_nat_inv i3). rewrite Hi3.
+                    rewrite <- of_nat_lt_sig1_neq. cbn. lia.
+                  * rewrite <- (of_nat_to_nat_inv i4). rewrite Hi4.
+                    rewrite <- of_nat_lt_sig1_neq in H4.
+                    rewrite <- of_nat_lt_sig1_neq. cbn. lia.
+                + assert (Hi0'' : S i0' < S (S n')) by lia.
+                  specialize (Hothers (of_nat_lt Hi0'')).
+                  do 2 (erewrite <- remove_vec_index_after; eauto).
+                  eapply Hothers; eauto.
+                  * rewrite <- (of_nat_to_nat_inv i3). rewrite Hi3.
+                    rewrite <- of_nat_lt_sig1_neq. cbn. lia.
+                  * rewrite <- (of_nat_to_nat_inv i4). rewrite Hi4.
+                    rewrite <- of_nat_lt_sig1_neq in H4.
+                    rewrite <- of_nat_lt_sig1_neq. cbn. lia.
+            }
+          }
+          (* i3' > i2', i4' < i2' *)
+          {
+            destruct i3'. inv H1.
+            assert (Hneq4: i3' <> i4').
+            {
+              rewrite <- (of_nat_to_nat_inv i3) in Hneq1. rewrite Hi3 in Hneq1.
+              rewrite <- (of_nat_to_nat_inv i4) in Hneq1. rewrite Hi4 in Hneq1.
+              rewrite <- of_nat_lt_sig1_neq in Hneq1. cbn in Hneq1. lia.
+            }
+            destruct (PeanoNat.Nat.eq_dec i' i3'); [| destruct (PeanoNat.Nat.eq_dec i' i4')].
+            {
+              (* we are going to i3' next *)
+              subst. rename Hi' into Hi3''.
+              assert (Hi4'' : i4' < S n') by lia.
+              apply trans_thread_schedule_val_SS with (i':=(of_nat_lt Hi4'')) in H.
+              eexists. apply H. rewrite Hequ. apply CIH; clear CIH. admit. admit.
+              right. right. split.
+              {
+                intro. eapply f_equal in H3. do 2 rewrite to_nat_of_nat in H3.
+                inv H3. contradiction.
+              }
+              split; [| split].
+              - rewrite <- (of_nat_to_nat_inv i2). rewrite Hi2. cbn.
+                assert (i3' = i2' \/ i3' > i2') by lia. destruct H3.
+                + erewrite <- remove_vec_index_eq; eauto.
+                  erewrite <- remove_vec_index_before; eauto.
+                  rewrite <- (of_nat_to_nat_inv i3) in Hi1sb.
+                  rewrite <- (of_nat_to_nat_inv i4) in Hi1sb.
+                  rewrite Hi3, Hi4 in Hi1sb. cbn in Hi1sb.
+                  apply Hi1sb.
+                + erewrite <- remove_vec_index_after; eauto.
+                  erewrite <- remove_vec_index_before; eauto.
+                  rewrite <- (of_nat_to_nat_inv i3) in Hi1sb.
+                  rewrite <- (of_nat_to_nat_inv i4) in Hi1sb.
+                  rewrite Hi3, Hi4 in Hi1sb. cbn in Hi1sb.
+                  apply Hi1sb.
+              - rewrite <- (of_nat_to_nat_inv i2). rewrite Hi2. cbn.
+                assert (i3' = i2' \/ i3' > i2') by lia. destruct H3.
+                + erewrite <- remove_vec_index_eq; eauto.
+                  erewrite <- remove_vec_index_before; eauto.
+                  rewrite <- (of_nat_to_nat_inv i3) in Hi2sb.
+                  rewrite <- (of_nat_to_nat_inv i4) in Hi2sb.
+                  rewrite Hi3, Hi4 in Hi2sb. cbn in Hi2sb.
+                  apply Hi2sb.
+                + erewrite <- remove_vec_index_after; eauto.
+                  erewrite <- remove_vec_index_before; eauto.
+                  rewrite <- (of_nat_to_nat_inv i3) in Hi2sb.
+                  rewrite <- (of_nat_to_nat_inv i4) in Hi2sb.
+                  rewrite Hi3, Hi4 in Hi2sb. cbn in Hi2sb.
+                  apply Hi2sb.
+              - intros.
+                destruct (to_nat i0) as [i0' Hi0'] eqn:Hi0.
+                rewrite <- (of_nat_to_nat_inv i2). rewrite Hi2.
+                rewrite <- (of_nat_to_nat_inv i0). rewrite Hi0. cbn.
+                rewrite <- (of_nat_to_nat_inv i0) in H3, H4. rewrite Hi0 in H3, H4. cbn in *.
+                assert (i0' < i2' \/ i0' = i2' \/ i0' > i2') by lia.
+                destruct H5 as [? | [? | ?]].
+                + assert (Hi0'' : i0' < S (S n')) by lia.
+                  specialize (Hothers (of_nat_lt Hi0'')).
+                  rewrite <- of_nat_lt_sig1_neq in H3.
+                  rewrite <- of_nat_lt_sig1_neq in H4.
+                  do 2 (erewrite <- remove_vec_index_before; eauto).
+                  eapply Hothers; eauto.
+                  * rewrite <- (of_nat_to_nat_inv i3). rewrite Hi3.
+                    rewrite <- of_nat_lt_sig1_neq. cbn. lia.
+                  * rewrite <- (of_nat_to_nat_inv i4). rewrite Hi4. cbn.
+                    rewrite <- of_nat_lt_sig1_neq. auto.
+                + subst. rename i2' into i0'.
+                  assert (Hi0'' : S i0' < S (S n')) by lia.
+                  specialize (Hothers (of_nat_lt Hi0'')).
+                  do 2 (erewrite <- remove_vec_index_eq; eauto).
+                  eapply Hothers; eauto.
+                  * rewrite <- (of_nat_to_nat_inv i3). rewrite Hi3.
+                    rewrite <- of_nat_lt_sig1_neq in H3.
+                    rewrite <- of_nat_lt_sig1_neq. cbn. lia.
+                  * rewrite <- (of_nat_to_nat_inv i4). rewrite Hi4.
+                    rewrite <- of_nat_lt_sig1_neq in H3.
+                    rewrite <- of_nat_lt_sig1_neq. cbn. lia.
+                + assert (Hi0'' : S i0' < S (S n')) by lia.
+                  specialize (Hothers (of_nat_lt Hi0'')).
+                  do 2 (erewrite <- remove_vec_index_after; eauto).
+                  eapply Hothers; eauto.
+                  * rewrite <- (of_nat_to_nat_inv i3). rewrite Hi3.
+                    rewrite <- of_nat_lt_sig1_neq in H3.
+                    rewrite <- of_nat_lt_sig1_neq. cbn. lia.
+                  * rewrite <- (of_nat_to_nat_inv i4). rewrite Hi4.
+                    rewrite <- of_nat_lt_sig1_neq. cbn. lia.
+            }
+            {
+              (* we are going to i4' next *)
+              subst. rename Hi' into Hi4''.
+              assert (Hi3'' : i3' < S n') by lia.
+              apply trans_thread_schedule_val_SS with (i':=(of_nat_lt Hi3'')) in H.
+              eexists. apply H. rewrite Hequ. apply CIH; clear CIH. admit. admit.
+              right. right. split.
+              {
+                intro. eapply f_equal in H3. do 2 rewrite to_nat_of_nat in H3.
+                inv H3. contradiction.
+              }
+              split; [| split].
+              - rewrite <- (of_nat_to_nat_inv i2). rewrite Hi2.
+                erewrite <- remove_vec_index_before; eauto.
+                assert (i3' = i2' \/ i3' > i2') by lia. destruct H3.
+                + subst. erewrite <- remove_vec_index_eq; eauto.
+                  rewrite <- (of_nat_to_nat_inv i3) in Hi2sb.
+                  rewrite <- (of_nat_to_nat_inv i4) in Hi2sb.
+                  rewrite Hi3, Hi4 in Hi2sb. cbn in Hi2sb.
+                  symmetry. apply Hi2sb.
+                + erewrite <- remove_vec_index_after; eauto.
+                  rewrite <- (of_nat_to_nat_inv i3) in Hi2sb.
+                  rewrite <- (of_nat_to_nat_inv i4) in Hi2sb.
+                  rewrite Hi3, Hi4 in Hi2sb. cbn in Hi2sb.
+                  symmetry. apply Hi2sb.
+              - rewrite <- (of_nat_to_nat_inv i2). rewrite Hi2. cbn.
+                erewrite <- remove_vec_index_before; eauto.
+                assert (i3' = i2' \/ i3' > i2') by lia. destruct H3.
+                + subst. erewrite <- remove_vec_index_eq; eauto.
+                  rewrite <- (of_nat_to_nat_inv i3) in Hi1sb.
+                  rewrite <- (of_nat_to_nat_inv i4) in Hi1sb.
+                  rewrite Hi3, Hi4 in Hi1sb. cbn in Hi1sb.
+                  symmetry. apply Hi1sb.
+                + erewrite <- remove_vec_index_after; eauto.
+                  rewrite <- (of_nat_to_nat_inv i3) in Hi1sb.
+                  rewrite <- (of_nat_to_nat_inv i4) in Hi1sb.
+                  rewrite Hi3, Hi4 in Hi1sb. cbn in Hi1sb.
+                  symmetry. apply Hi1sb.
+              - intros.
+                destruct (to_nat i0) as [i0' Hi0'] eqn:Hi0.
+                rewrite <- (of_nat_to_nat_inv i2). rewrite Hi2.
+                rewrite <- (of_nat_to_nat_inv i0). rewrite Hi0. cbn.
+                rewrite <- (of_nat_to_nat_inv i0) in H3, H4. rewrite Hi0 in H3, H4. cbn in *.
+                assert (i0' < i2' \/ i0' = i2' \/ i0' > i2') by lia.
+                destruct H5 as [? | [? | ?]].
+                + assert (Hi0'' : i0' < S (S n')) by lia.
+                  specialize (Hothers (of_nat_lt Hi0'')).
+                  rewrite <- of_nat_lt_sig1_neq in H3.
+                  rewrite <- of_nat_lt_sig1_neq in H4.
+                  do 2 (erewrite <- remove_vec_index_before; eauto).
+                  eapply Hothers; eauto.
+                  * rewrite <- (of_nat_to_nat_inv i3). rewrite Hi3.
+                    rewrite <- of_nat_lt_sig1_neq. cbn. lia.
+                  * rewrite <- (of_nat_to_nat_inv i4). rewrite Hi4. cbn.
+                    rewrite <- of_nat_lt_sig1_neq. auto.
+                + subst. rename i2' into i0'.
+                  assert (Hi0'' : S i0' < S (S n')) by lia.
+                  specialize (Hothers (of_nat_lt Hi0'')).
+                  do 2 (erewrite <- remove_vec_index_eq; eauto).
+                  eapply Hothers; eauto.
+                  * rewrite <- (of_nat_to_nat_inv i3). rewrite Hi3.
+                    rewrite <- of_nat_lt_sig1_neq in H4.
+                    rewrite <- of_nat_lt_sig1_neq. cbn. lia.
+                  * rewrite <- (of_nat_to_nat_inv i4). rewrite Hi4.
+                    rewrite <- of_nat_lt_sig1_neq. cbn. lia.
+                + assert (Hi0'' : S i0' < S (S n')) by lia.
+                  specialize (Hothers (of_nat_lt Hi0'')).
+                  do 2 (erewrite <- remove_vec_index_after; eauto).
+                  eapply Hothers; eauto.
+                  * rewrite <- (of_nat_to_nat_inv i3). rewrite Hi3.
+                    rewrite <- of_nat_lt_sig1_neq in H4.
+                    rewrite <- of_nat_lt_sig1_neq. cbn. lia.
+                  * rewrite <- (of_nat_to_nat_inv i4). rewrite Hi4.
+                    rewrite <- of_nat_lt_sig1_neq. cbn. lia.
+            }
+            {
+              (* we are going to i', which is not one of the swapped elements *)
+              assert (Hi3'' : i3' < S n') by lia.
+              assert (Hi4'' : i4' < S n') by lia.
+              apply trans_thread_schedule_val_SS with (i':=(of_nat_lt Hi')) in H.
+              eexists. apply H. rewrite Hequ. apply CIH; clear CIH. admit. admit.
+              right. left. split; auto.
+              exists (of_nat_lt Hi3''), (of_nat_lt Hi4'').
+              split; [| split; [| split]]; try solve [rewrite <- of_nat_lt_sig1_neq; auto].
+              split; [| split].
+              - rewrite <- (of_nat_to_nat_inv i2). rewrite Hi2. cbn.
+                assert (i3' = i2' \/ i3' > i2') by lia. destruct H3.
+                + subst. erewrite <- remove_vec_index_eq; eauto.
+                  erewrite <- remove_vec_index_before; eauto.
+                  rewrite <- (of_nat_to_nat_inv i3) in Hi1sb.
+                  rewrite <- (of_nat_to_nat_inv i4) in Hi1sb.
+                  rewrite Hi3, Hi4 in Hi1sb. cbn in Hi1sb.
+                  apply Hi1sb.
+                + erewrite <- remove_vec_index_after; eauto.
+                  erewrite <- remove_vec_index_before; eauto.
+                  rewrite <- (of_nat_to_nat_inv i3) in Hi1sb.
+                  rewrite <- (of_nat_to_nat_inv i4) in Hi1sb.
+                  rewrite Hi3, Hi4 in Hi1sb. cbn in Hi1sb.
+                  apply Hi1sb.
+              - rewrite <- (of_nat_to_nat_inv i2). rewrite Hi2. cbn.
+                assert (i3' = i2' \/ i3' > i2') by lia. destruct H3.
+                + subst. erewrite <- remove_vec_index_eq; eauto.
+                  erewrite <- remove_vec_index_before; eauto.
+                  rewrite <- (of_nat_to_nat_inv i3) in Hi2sb.
+                  rewrite <- (of_nat_to_nat_inv i4) in Hi2sb.
+                  rewrite Hi3, Hi4 in Hi2sb. cbn in Hi2sb.
+                  apply Hi2sb.
+                + erewrite <- remove_vec_index_after; eauto.
+                  erewrite <- remove_vec_index_before; eauto.
+                  rewrite <- (of_nat_to_nat_inv i3) in Hi2sb.
+                  rewrite <- (of_nat_to_nat_inv i4) in Hi2sb.
+                  rewrite Hi3, Hi4 in Hi2sb. cbn in Hi2sb.
+                  apply Hi2sb.
+              - intros.
+                destruct (to_nat i0) as [i0' Hi0'] eqn:Hi0.
+                rewrite <- (of_nat_to_nat_inv i2). rewrite Hi2.
+                rewrite <- (of_nat_to_nat_inv i0). rewrite Hi0. cbn.
+                rewrite <- (of_nat_to_nat_inv i0) in H3, H4. rewrite Hi0 in H3, H4. cbn in *.
+                assert (i0' < i2' \/ i0' = i2' \/ i0' > i2') by lia.
+                destruct H5 as [? | [? | ?]].
+                + assert (Hi0'' : i0' < S (S n')) by lia.
+                  specialize (Hothers (of_nat_lt Hi0'')).
+                  rewrite <- of_nat_lt_sig1_neq in H3.
+                  rewrite <- of_nat_lt_sig1_neq in H4.
+                  do 2 (erewrite <- remove_vec_index_before; eauto).
+                  eapply Hothers; eauto.
+                  * rewrite <- (of_nat_to_nat_inv i3). rewrite Hi3.
+                    rewrite <- of_nat_lt_sig1_neq. cbn. lia.
+                  * rewrite <- (of_nat_to_nat_inv i4). rewrite Hi4. cbn.
+                    rewrite <- of_nat_lt_sig1_neq. auto.
+                + subst. rename i2' into i0'.
+                  assert (Hi0'' : S i0' < S (S n')) by lia.
+                  specialize (Hothers (of_nat_lt Hi0'')).
+                  do 2 (erewrite <- remove_vec_index_eq; eauto).
+                  eapply Hothers; eauto.
+                  * rewrite <- (of_nat_to_nat_inv i3). rewrite Hi3.
+                    rewrite <- of_nat_lt_sig1_neq in H3.
+                    rewrite <- of_nat_lt_sig1_neq. cbn. lia.
+                  * rewrite <- (of_nat_to_nat_inv i4). rewrite Hi4.
+                    rewrite <- of_nat_lt_sig1_neq. cbn. lia.
+                + assert (Hi0'' : S i0' < S (S n')) by lia.
+                  specialize (Hothers (of_nat_lt Hi0'')).
+                  do 2 (erewrite <- remove_vec_index_after; eauto).
+                  eapply Hothers; eauto.
+                  * rewrite <- (of_nat_to_nat_inv i3). rewrite Hi3.
+                    rewrite <- of_nat_lt_sig1_neq in H3.
+                    rewrite <- of_nat_lt_sig1_neq. cbn. lia.
+                  * rewrite <- (of_nat_to_nat_inv i4). rewrite Hi4.
+                    rewrite <- of_nat_lt_sig1_neq. cbn. lia.
+            }
+          }
+          (* i3' > i2', i4' > i2' *)
+          {
+            destruct i3'. inv H1.
+            destruct i4'. inv H2.
+            assert (Hneq4: i3' <> i4').
+            {
+              rewrite <- (of_nat_to_nat_inv i3) in Hneq1. rewrite Hi3 in Hneq1.
+              rewrite <- (of_nat_to_nat_inv i4) in Hneq1. rewrite Hi4 in Hneq1.
+              rewrite <- of_nat_lt_sig1_neq in Hneq1. cbn in Hneq1. lia.
+            }
+
+            destruct (PeanoNat.Nat.eq_dec i' i3'); [| destruct (PeanoNat.Nat.eq_dec i' i4')].
+            {
+              (* we are going to i3' next *)
+              subst. rename Hi' into Hi3''.
+              (* destruct i4'. inv H2. (* subtract i4' by one *) *)
+              assert (Hi4'' : i4' < S n') by lia.
+              apply trans_thread_schedule_val_SS with (i':=(of_nat_lt Hi4'')) in H.
+              eexists. apply H. rewrite Hequ. apply CIH; clear CIH. admit. admit.
+              right. right. split.
+              {
+                intro. eapply f_equal in H3. do 2 rewrite to_nat_of_nat in H3.
+                inv H3. contradiction.
+              }
+              split; [| split].
+              - rewrite <- (of_nat_to_nat_inv i2). rewrite Hi2. cbn.
+                assert (i3' = i2' \/ i3' > i2') by lia.
+                assert (i4' = i2' \/ i4' > i2') by lia. destruct H3, H4.
+                + do 2 (erewrite <- remove_vec_index_eq; eauto).
+                  rewrite <- (of_nat_to_nat_inv i3) in Hi1sb.
+                  rewrite <- (of_nat_to_nat_inv i4) in Hi1sb.
+                  rewrite Hi3, Hi4 in Hi1sb. cbn in Hi1sb.
+                  apply Hi1sb.
+                + erewrite <- remove_vec_index_eq; eauto.
+                  erewrite <- remove_vec_index_after; eauto.
+                  rewrite <- (of_nat_to_nat_inv i3) in Hi1sb.
+                  rewrite <- (of_nat_to_nat_inv i4) in Hi1sb.
+                  rewrite Hi3, Hi4 in Hi1sb. cbn in Hi1sb.
+                  apply Hi1sb.
+                + erewrite <- remove_vec_index_after; eauto.
+                  erewrite <- remove_vec_index_eq; eauto.
+                  rewrite <- (of_nat_to_nat_inv i3) in Hi1sb.
+                  rewrite <- (of_nat_to_nat_inv i4) in Hi1sb.
+                  rewrite Hi3, Hi4 in Hi1sb. cbn in Hi1sb.
+                  apply Hi1sb.
+                + do 2 (erewrite <- remove_vec_index_after; eauto).
+                  rewrite <- (of_nat_to_nat_inv i3) in Hi1sb.
+                  rewrite <- (of_nat_to_nat_inv i4) in Hi1sb.
+                  rewrite Hi3, Hi4 in Hi1sb. cbn in Hi1sb.
+                  apply Hi1sb.
+              - rewrite <- (of_nat_to_nat_inv i2). rewrite Hi2. cbn.
+                assert (i3' = i2' \/ i3' > i2') by lia.
+                assert (i4' = i2' \/ i4' > i2') by lia. destruct H3, H4.
+                + do 2 (erewrite <- remove_vec_index_eq; eauto).
+                  rewrite <- (of_nat_to_nat_inv i3) in Hi2sb.
+                  rewrite <- (of_nat_to_nat_inv i4) in Hi2sb.
+                  rewrite Hi3, Hi4 in Hi2sb. cbn in Hi2sb.
+                  apply Hi2sb.
+                + erewrite <- remove_vec_index_eq; eauto.
+                  erewrite <- remove_vec_index_after; eauto.
+                  rewrite <- (of_nat_to_nat_inv i3) in Hi2sb.
+                  rewrite <- (of_nat_to_nat_inv i4) in Hi2sb.
+                  rewrite Hi3, Hi4 in Hi2sb. cbn in Hi2sb.
+                  apply Hi2sb.
+                + erewrite <- remove_vec_index_after; eauto.
+                  erewrite <- remove_vec_index_eq; eauto.
+                  rewrite <- (of_nat_to_nat_inv i3) in Hi2sb.
+                  rewrite <- (of_nat_to_nat_inv i4) in Hi2sb.
+                  rewrite Hi3, Hi4 in Hi2sb. cbn in Hi2sb.
+                  apply Hi2sb.
+                + do 2 (erewrite <- remove_vec_index_after; eauto).
+                  rewrite <- (of_nat_to_nat_inv i3) in Hi2sb.
+                  rewrite <- (of_nat_to_nat_inv i4) in Hi2sb.
+                  rewrite Hi3, Hi4 in Hi2sb. cbn in Hi2sb.
+                  apply Hi2sb.
+              - intros.
+                destruct (to_nat i0) as [i0' Hi0'] eqn:Hi0.
+                rewrite <- (of_nat_to_nat_inv i2). rewrite Hi2.
+                rewrite <- (of_nat_to_nat_inv i0). rewrite Hi0. cbn.
+                rewrite <- (of_nat_to_nat_inv i0) in H3, H4. rewrite Hi0 in H3, H4. cbn in *.
+                assert (i0' < i2' \/ i0' = i2' \/ i0' > i2') by lia.
+                destruct H5 as [? | [? | ?]].
+                + assert (Hi0'' : i0' < S (S n')) by lia.
+                  specialize (Hothers (of_nat_lt Hi0'')).
+                  rewrite <- of_nat_lt_sig1_neq in H3.
+                  rewrite <- of_nat_lt_sig1_neq in H4.
+                  do 2 (erewrite <- remove_vec_index_before; eauto).
+                  eapply Hothers; eauto.
+                  * rewrite <- (of_nat_to_nat_inv i3). rewrite Hi3.
+                    rewrite <- of_nat_lt_sig1_neq. cbn. lia.
+                  * rewrite <- (of_nat_to_nat_inv i4). rewrite Hi4.
+                    rewrite <- of_nat_lt_sig1_neq. cbn. lia.
+                + subst. rename i2' into i0'.
+                  assert (Hi0'' : S i0' < S (S n')) by lia.
+                  specialize (Hothers (of_nat_lt Hi0'')).
+                  do 2 (erewrite <- remove_vec_index_eq; eauto).
+                  eapply Hothers; eauto.
+                  * rewrite <- (of_nat_to_nat_inv i3). rewrite Hi3.
+                    rewrite <- of_nat_lt_sig1_neq in H3.
+                    rewrite <- of_nat_lt_sig1_neq. cbn. lia.
+                  * rewrite <- (of_nat_to_nat_inv i4). rewrite Hi4.
+                    rewrite <- of_nat_lt_sig1_neq in H4.
+                    rewrite <- of_nat_lt_sig1_neq. cbn. lia.
+                + assert (Hi0'' : S i0' < S (S n')) by lia.
+                  specialize (Hothers (of_nat_lt Hi0'')).
+                  do 2 (erewrite <- remove_vec_index_after; eauto).
+                  eapply Hothers; eauto.
+                  * rewrite <- (of_nat_to_nat_inv i3). rewrite Hi3.
+                    rewrite <- of_nat_lt_sig1_neq in H3.
+                    rewrite <- of_nat_lt_sig1_neq. cbn. lia.
+                  * rewrite <- (of_nat_to_nat_inv i4). rewrite Hi4.
+                    rewrite <- of_nat_lt_sig1_neq in H4.
+                    rewrite <- of_nat_lt_sig1_neq. cbn. lia.
+            }
+            {
+              (* we are going to i4' next *)
+              subst. rename Hi' into Hi4''.
+              assert (Hi3'' : i3' < S n') by lia.
+              apply trans_thread_schedule_val_SS with (i':=(of_nat_lt Hi3'')) in H.
+              eexists. apply H. rewrite Hequ. apply CIH; clear CIH. admit. admit.
+              right. right. split.
+              {
+                intro. eapply f_equal in H3. do 2 rewrite to_nat_of_nat in H3.
+                inv H3. contradiction.
+              }
+              split; [| split].
+              - rewrite <- (of_nat_to_nat_inv i2). rewrite Hi2.
+                assert (i4' = i2' \/ i4' > i2') by lia.
+                assert (i3' = i2' \/ i3' > i2') by lia. destruct H3, H4.
+                + do 2 (erewrite <- remove_vec_index_eq; eauto).
+                  rewrite <- (of_nat_to_nat_inv i3) in Hi2sb.
+                  rewrite <- (of_nat_to_nat_inv i4) in Hi2sb.
+                  rewrite Hi3, Hi4 in Hi2sb. cbn in Hi2sb.
+                  symmetry. eapply Hi2sb.
+                + erewrite <- remove_vec_index_eq; eauto.
+                  erewrite <- remove_vec_index_after; eauto.
+                  rewrite <- (of_nat_to_nat_inv i3) in Hi2sb.
+                  rewrite <- (of_nat_to_nat_inv i4) in Hi2sb.
+                  rewrite Hi3, Hi4 in Hi2sb. cbn in Hi2sb.
+                  symmetry. eapply Hi2sb.
+                + erewrite <- remove_vec_index_after; eauto.
+                  erewrite <- remove_vec_index_eq; eauto.
+                  rewrite <- (of_nat_to_nat_inv i3) in Hi2sb.
+                  rewrite <- (of_nat_to_nat_inv i4) in Hi2sb.
+                  rewrite Hi3, Hi4 in Hi2sb. cbn in Hi2sb.
+                  symmetry. eapply Hi2sb.
+                + do 2 (erewrite <- remove_vec_index_after; eauto).
+                  rewrite <- (of_nat_to_nat_inv i3) in Hi2sb.
+                  rewrite <- (of_nat_to_nat_inv i4) in Hi2sb.
+                  rewrite Hi3, Hi4 in Hi2sb. cbn in Hi2sb.
+                  symmetry. eapply Hi2sb.
+              - rewrite <- (of_nat_to_nat_inv i2). rewrite Hi2. cbn.
+                assert (i4' = i2' \/ i4' > i2') by lia.
+                assert (i3' = i2' \/ i3' > i2') by lia. destruct H3, H4.
+                + do 2 (erewrite <- remove_vec_index_eq; eauto).
+                  rewrite <- (of_nat_to_nat_inv i3) in Hi1sb.
+                  rewrite <- (of_nat_to_nat_inv i4) in Hi1sb.
+                  rewrite Hi3, Hi4 in Hi1sb. cbn in Hi1sb.
+                  symmetry. eapply Hi1sb.
+                + erewrite <- remove_vec_index_eq; eauto.
+                  erewrite <- remove_vec_index_after; eauto.
+                  rewrite <- (of_nat_to_nat_inv i3) in Hi1sb.
+                  rewrite <- (of_nat_to_nat_inv i4) in Hi1sb.
+                  rewrite Hi3, Hi4 in Hi1sb. cbn in Hi1sb.
+                  symmetry. eapply Hi1sb.
+                + erewrite <- remove_vec_index_after; eauto.
+                  erewrite <- remove_vec_index_eq; eauto.
+                  rewrite <- (of_nat_to_nat_inv i3) in Hi1sb.
+                  rewrite <- (of_nat_to_nat_inv i4) in Hi1sb.
+                  rewrite Hi3, Hi4 in Hi1sb. cbn in Hi1sb.
+                  symmetry. eapply Hi1sb.
+                + do 2 (erewrite <- remove_vec_index_after; eauto).
+                  rewrite <- (of_nat_to_nat_inv i3) in Hi1sb.
+                  rewrite <- (of_nat_to_nat_inv i4) in Hi1sb.
+                  rewrite Hi3, Hi4 in Hi1sb. cbn in Hi1sb.
+                  symmetry. eapply Hi1sb.
+              - intros.
+                destruct (to_nat i0) as [i0' Hi0'] eqn:Hi0.
+                rewrite <- (of_nat_to_nat_inv i2). rewrite Hi2.
+                rewrite <- (of_nat_to_nat_inv i0). rewrite Hi0. cbn.
+                rewrite <- (of_nat_to_nat_inv i0) in H3, H4. rewrite Hi0 in H3, H4. cbn in *.
+                assert (i0' < i2' \/ i0' = i2' \/ i0' > i2') by lia.
+                destruct H5 as [? | [? | ?]].
+                + assert (Hi0'' : i0' < S (S n')) by lia.
+                  specialize (Hothers (of_nat_lt Hi0'')).
+                  rewrite <- of_nat_lt_sig1_neq in H3.
+                  rewrite <- of_nat_lt_sig1_neq in H4.
+                  do 2 (erewrite <- remove_vec_index_before; eauto).
+                  eapply Hothers; eauto.
+                  * rewrite <- (of_nat_to_nat_inv i3). rewrite Hi3.
+                    rewrite <- of_nat_lt_sig1_neq. cbn. lia.
+                  * rewrite <- (of_nat_to_nat_inv i4). rewrite Hi4.
+                    rewrite <- of_nat_lt_sig1_neq. cbn. lia.
+                + subst. rename i2' into i0'.
+                  assert (Hi0'' : S i0' < S (S n')) by lia.
+                  specialize (Hothers (of_nat_lt Hi0'')).
+                  do 2 (erewrite <- remove_vec_index_eq; eauto).
+                  eapply Hothers; eauto.
+                  * rewrite <- (of_nat_to_nat_inv i3). rewrite Hi3.
+                    rewrite <- of_nat_lt_sig1_neq in H4.
+                    rewrite <- of_nat_lt_sig1_neq. cbn. lia.
+                  * rewrite <- (of_nat_to_nat_inv i4). rewrite Hi4.
+                    rewrite <- of_nat_lt_sig1_neq in H3.
+                    rewrite <- of_nat_lt_sig1_neq. cbn. lia.
+                + assert (Hi0'' : S i0' < S (S n')) by lia.
+                  specialize (Hothers (of_nat_lt Hi0'')).
+                  do 2 (erewrite <- remove_vec_index_after; eauto).
+                  eapply Hothers; eauto.
+                  * rewrite <- (of_nat_to_nat_inv i3). rewrite Hi3.
+                    rewrite <- of_nat_lt_sig1_neq in H4.
+                    rewrite <- of_nat_lt_sig1_neq. cbn. lia.
+                  * rewrite <- (of_nat_to_nat_inv i4). rewrite Hi4.
+                    rewrite <- of_nat_lt_sig1_neq in H3.
+                    rewrite <- of_nat_lt_sig1_neq. cbn. lia.
+            }
+            {
+              (* we are going to i', which is not one of the swapped elements *)
+              assert (Hi3'' : i3' < S n') by lia.
+              assert (Hi4'' : i4' < S n') by lia.
+              apply trans_thread_schedule_val_SS with (i':=(of_nat_lt Hi')) in H.
+              eexists. apply H. rewrite Hequ. apply CIH; clear CIH. admit. admit.
+              right. left. split; auto.
+              exists (of_nat_lt Hi3''), (of_nat_lt Hi4'').
+              split; [| split; [| split]]; try solve [rewrite <- of_nat_lt_sig1_neq; auto].
+              split; [| split].
+              - rewrite <- (of_nat_to_nat_inv i2). rewrite Hi2. cbn.
+                assert (i3' = i2' \/ i3' > i2') by lia.
+                assert (i4' = i2' \/ i4' > i2') by lia. destruct H3, H4.
+                + do 2 (erewrite <- remove_vec_index_eq; eauto).
+                  rewrite <- (of_nat_to_nat_inv i3) in Hi1sb.
+                  rewrite <- (of_nat_to_nat_inv i4) in Hi1sb.
+                  rewrite Hi3, Hi4 in Hi1sb. cbn in Hi1sb.
+                  apply Hi1sb.
+                + erewrite <- remove_vec_index_eq; eauto.
+                  erewrite <- remove_vec_index_after; eauto.
+                  rewrite <- (of_nat_to_nat_inv i3) in Hi1sb.
+                  rewrite <- (of_nat_to_nat_inv i4) in Hi1sb.
+                  rewrite Hi3, Hi4 in Hi1sb. cbn in Hi1sb.
+                  apply Hi1sb.
+                + erewrite <- remove_vec_index_after; eauto.
+                  erewrite <- remove_vec_index_eq; eauto.
+                  rewrite <- (of_nat_to_nat_inv i3) in Hi1sb.
+                  rewrite <- (of_nat_to_nat_inv i4) in Hi1sb.
+                  rewrite Hi3, Hi4 in Hi1sb. cbn in Hi1sb.
+                  apply Hi1sb.
+                + do 2 (erewrite <- remove_vec_index_after; eauto).
+                  rewrite <- (of_nat_to_nat_inv i3) in Hi1sb.
+                  rewrite <- (of_nat_to_nat_inv i4) in Hi1sb.
+                  rewrite Hi3, Hi4 in Hi1sb. cbn in Hi1sb.
+                  apply Hi1sb.
+              - rewrite <- (of_nat_to_nat_inv i2). rewrite Hi2. cbn.
+                assert (i3' = i2' \/ i3' > i2') by lia.
+                assert (i4' = i2' \/ i4' > i2') by lia. destruct H3, H4.
+                + do 2 (erewrite <- remove_vec_index_eq; eauto).
+                  rewrite <- (of_nat_to_nat_inv i3) in Hi2sb.
+                  rewrite <- (of_nat_to_nat_inv i4) in Hi2sb.
+                  rewrite Hi3, Hi4 in Hi2sb. cbn in Hi2sb.
+                  apply Hi2sb.
+                + erewrite <- remove_vec_index_eq; eauto.
+                  erewrite <- remove_vec_index_after; eauto.
+                  rewrite <- (of_nat_to_nat_inv i3) in Hi2sb.
+                  rewrite <- (of_nat_to_nat_inv i4) in Hi2sb.
+                  rewrite Hi3, Hi4 in Hi2sb. cbn in Hi2sb.
+                  apply Hi2sb.
+                + erewrite <- remove_vec_index_after; eauto.
+                  erewrite <- remove_vec_index_eq; eauto.
+                  rewrite <- (of_nat_to_nat_inv i3) in Hi2sb.
+                  rewrite <- (of_nat_to_nat_inv i4) in Hi2sb.
+                  rewrite Hi3, Hi4 in Hi2sb. cbn in Hi2sb.
+                  apply Hi2sb.
+                + do 2 (erewrite <- remove_vec_index_after; eauto).
+                  rewrite <- (of_nat_to_nat_inv i3) in Hi2sb.
+                  rewrite <- (of_nat_to_nat_inv i4) in Hi2sb.
+                  rewrite Hi3, Hi4 in Hi2sb. cbn in Hi2sb.
+                  apply Hi2sb.
+              - intros.
+                destruct (to_nat i0) as [i0' Hi0'] eqn:Hi0.
+                rewrite <- (of_nat_to_nat_inv i2). rewrite Hi2.
+                rewrite <- (of_nat_to_nat_inv i0). rewrite Hi0. cbn.
+                rewrite <- (of_nat_to_nat_inv i0) in H3, H4. rewrite Hi0 in H3, H4. cbn in *.
+                assert (i0' < i2' \/ i0' = i2' \/ i0' > i2') by lia.
+                destruct H5 as [? | [? | ?]].
+                + assert (Hi0'' : i0' < S (S n')) by lia.
+                  specialize (Hothers (of_nat_lt Hi0'')).
+                  rewrite <- of_nat_lt_sig1_neq in H3.
+                  rewrite <- of_nat_lt_sig1_neq in H4.
+                  do 2 (erewrite <- remove_vec_index_before; eauto).
+                  eapply Hothers; eauto.
+                  * rewrite <- (of_nat_to_nat_inv i3). rewrite Hi3.
+                    rewrite <- of_nat_lt_sig1_neq. cbn. lia.
+                  * rewrite <- (of_nat_to_nat_inv i4). rewrite Hi4.
+                    rewrite <- of_nat_lt_sig1_neq. cbn. lia.
+                + subst. rename i2' into i0'.
+                  assert (Hi0'' : S i0' < S (S n')) by lia.
+                  specialize (Hothers (of_nat_lt Hi0'')).
+                  do 2 (erewrite <- remove_vec_index_eq; eauto).
+                  eapply Hothers; eauto.
+                  * rewrite <- (of_nat_to_nat_inv i3). rewrite Hi3.
+                    rewrite <- of_nat_lt_sig1_neq in H3.
+                    rewrite <- of_nat_lt_sig1_neq. cbn. lia.
+                  * rewrite <- (of_nat_to_nat_inv i4). rewrite Hi4.
+                    rewrite <- of_nat_lt_sig1_neq in H4.
+                    rewrite <- of_nat_lt_sig1_neq. cbn. lia.
+                + assert (Hi0'' : S i0' < S (S n')) by lia.
+                  specialize (Hothers (of_nat_lt Hi0'')).
+                  do 2 (erewrite <- remove_vec_index_after; eauto).
+                  eapply Hothers; eauto.
+                  * rewrite <- (of_nat_to_nat_inv i3). rewrite Hi3.
+                    rewrite <- of_nat_lt_sig1_neq in H3.
+                    rewrite <- of_nat_lt_sig1_neq. cbn. lia.
+                  * rewrite <- (of_nat_to_nat_inv i4). rewrite Hi4.
+                    rewrite <- of_nat_lt_sig1_neq in H4.
+                    rewrite <- of_nat_lt_sig1_neq. cbn. lia.
+            }
+          }
+        * (* the finished thread is one of the swapped threads. this can lead to there still being 2 swapped threads, or no swapped threads, depending on the positions of the two threads *)
+          rewrite <- (of_nat_to_nat_inv i) in Hequ. rewrite <- (of_nat_to_nat_inv i1) in Hequ.
+          destruct (to_nat i) as [i' Hi'] eqn:Hi.
+          destruct (to_nat i1) as [i1' Hi1'] eqn:Hi1. cbn in Hequ.
+          destruct (to_nat i2) as [i2' Hi2'] eqn:Hi2.
+          pose proof Hi1sb.
+          step in H. destruct H as [Hf _].
+          edestruct Hf as [? ? ?]; eauto.
+          assert (i1' <> i2') by admit.
+          assert (i1' = S i2' \/ i2' =  S i1' \/ S i1' < i2' \/ S i2' < i1') by lia.
+          destruct H2 as [? | [? | [? | ?]]].
+          -- (* | i2 | i1 |, no more swapped elements *)
+            subst.
+            assert (i' < i2' \/ i' = i2' \/ i' > i2') by lia. destruct H2.
+            ++ eapply trans_thread_schedule_val_SS with (i':=(of_nat_lt Hi')) in H.
+               eexists. apply H. rewrite Hequ. apply CIH; clear CIH. admit. admit.
+               left. split; auto.
+               intros. rewrite <- (of_nat_to_nat_inv i2). rewrite Hi2.
+             assert (i4' < i2' \/ i4' > i2').
+             cbn.
+          -- (* | i1 | i2 |, no more swapped elements *)
+          -- (* | i1 | ... | i2 |, still swapped elements *)
+          -- (* | i2 | ... | i1 | *)
+
+          (* copy struct from prev case, do case analysis on top level, then
+             do case analysis here on what i is *)
+
+          eapply trans_thread_schedule_val_SS with (i':=(of_nat_lt Hi')) in H.
+          eexists. apply H. rewrite Hequ. apply CIH; clear CIH. admit. admit.
+
+
+          (* we just removed one of the swapped ones, so now it can either be all in order or there can still be one swapped.... *)
+          (* right. left. split; auto.  *)
+          left. split; eauto.
+          intros. admit.
+      + (* tau step *)
+        destruct n; try inv i1.
+        destruct H0 as (t' & Ht & Hbound & Hequ).
+        destruct Hi as [
+            (? & Hv) | [
+              (? & i3 & i4 & Hneq1 & Hneq2 & Hneq3 & Hi1sb & Hi2sb & Hothers) |
+              (Hneq & Hi1sb & Hi2sb & Hothers)]].
+        * subst. pose proof (Hv i2). step in H. destruct H as [Hf _].
+          edestruct Hf as [? ? ?]; eauto.
+          epose proof (trans_choiceI_bound _ _ _ _ _ H).
+          apply trans_thread_schedule_tau in H.
+          eexists; eauto. rewrite Hequ. apply CIH. admit. admit.
+          left. split; auto.
+          intros. destruct (Fin.eq_dec i i2).
+          -- subst. do 2 rewrite replace_vec_eq. auto.
+          -- do 2 (rewrite replace_vec_neq; auto).
+        * subst. epose proof (Hothers i2 _ _); eauto. step in H. destruct H as [Hf _].
+          edestruct Hf as [? ? ?]; eauto.
+          epose proof (trans_choiceI_bound _ _ _ _ _ H).
+          apply trans_thread_schedule_tau in H.
+          eexists; eauto. rewrite Hequ. apply CIH. admit. admit.
+          right. left. split; auto. exists i3, i4. split; [| split; [| split]]; auto.
+          split; [| split].
+          -- do 2 (rewrite replace_vec_neq; auto).
+          -- do 2 (rewrite replace_vec_neq; auto).
+          -- intros. destruct (Fin.eq_dec i i2).
+             ++ subst. do 2 rewrite replace_vec_eq; auto.
+             ++ do 2 (rewrite replace_vec_neq; auto); auto.
+        * step in Hi1sb. destruct Hi1sb as [Hf _].
+          edestruct Hf as [? ? ?]; eauto.
+          epose proof (trans_choiceI_bound _ _ _ _ _ H).
+          apply trans_thread_schedule_tau in H.
+          eexists; eauto. rewrite Hequ. apply CIH. admit. admit.
+          right. right. split; auto.
+          split; [| split].
+          -- do 2 rewrite replace_vec_eq; auto.
+          -- do 2 (rewrite replace_vec_neq; auto).
+          -- intros. do 2 (rewrite replace_vec_neq; auto).
+      + (* The thread yields *)
+        destruct H as (k & Hvis & i' & Hequ).
+        destruct Hi as [
+            (? & Hv) | [
+              (? & i3 & i4 & Hneq1 & Hneq2 & Hneq3 & Hi1sb & Hi2sb & Hothers) |
+              (Hneq & Hi1sb & Hi2sb & Hothers)]].
+        * subst. destruct n; try inv i2.
+          pose proof Hvis as Hvis'.
+          eapply sbisim_visible in Hvis'. 5: apply Hv. all: auto.
+          destruct Hvis' as (k' & Hvis' & Hk).
+          exists (schedule (S n) (replace_vec v2 i2 (k' tt)) (Some i')).
+          2: { rewrite Hequ. apply CIH. admit. admit.
+               left. split; auto. intros.
+               apply replace_vec_vec_relation; auto.
+          }
+          apply visible_yield_trans_schedule; auto.
+        * subst. destruct n; try inv i2.
+          pose proof Hvis as Hvis'.
+          eapply sbisim_visible in Hvis'. 5: apply Hothers; auto. all: auto.
+          destruct Hvis' as (k' & Hvis' & Hk).
+          destruct (Fin.eq_dec i' i3); [| destruct (Fin.eq_dec i' i4)]; subst.
+          -- (* we are going to i3 *)
+            exists (schedule (S n) (replace_vec v2 i2 (k' tt)) (Some i4)).
+            2: { rewrite Hequ. apply CIH. admit. admit.
+                 right. right. split; auto. split; [| split]; auto.
+                 - do 2 (rewrite replace_vec_neq; auto).
+                 - do 2 (rewrite replace_vec_neq; auto).
+                 - intros. destruct (Fin.eq_dec i2 i).
+                   + subst. do 2 (rewrite replace_vec_eq; auto).
+                   + do 2 (rewrite replace_vec_neq; auto).
+            }
+          apply visible_yield_trans_schedule; auto.
+          -- (* we are going to i4 *)
+            exists (schedule (S n) (replace_vec v2 i2 (k' tt)) (Some i3)).
+            2: { rewrite Hequ. apply CIH. admit. admit.
+                 right. right. split; auto. split; [| split]; auto.
+                 - do 2 (rewrite replace_vec_neq; auto). symmetry; auto.
+                 - do 2 (rewrite replace_vec_neq; auto). symmetry; auto.
+                 - intros. destruct (Fin.eq_dec i2 i).
+                   + subst. do 2 (rewrite replace_vec_eq; auto).
+                   + do 2 (rewrite replace_vec_neq; auto).
+            }
+            apply visible_yield_trans_schedule; auto.
+          -- (* we are not going to a swapped element *)
+            exists (schedule (S n) (replace_vec v2 i2 (k' tt)) (Some i')).
+            2: { rewrite Hequ. apply CIH. admit. admit.
+                 right. left. split; auto. exists i3, i4. split; [| split; [| split]]; auto.
+                 split; [| split]; auto.
+                 - do 2 (rewrite replace_vec_neq; auto).
+                 - do 2 (rewrite replace_vec_neq; auto).
+                 - intros. destruct (Fin.eq_dec i2 i).
+                   + subst. do 2 (rewrite replace_vec_eq; auto).
+                   + do 2 (rewrite replace_vec_neq; auto).
+            }
+            apply visible_yield_trans_schedule; auto.
+        * destruct n; try inv i2.
+          pose proof Hvis as Hvis'.
+          eapply sbisim_visible in Hvis'. 5: apply Hi1sb. all: auto.
+          destruct Hvis' as (k' & Hvis' & Hk).
+          destruct (Fin.eq_dec i' i1); [| destruct (Fin.eq_dec i' i2)]; subst.
+          -- (* going to i1 *)
+            exists (schedule (S n) (replace_vec v2 i2 (k' tt)) (Some i2)).
+            2: { rewrite Hequ. apply CIH. admit. admit.
+                 right. right. split; auto. split; [| split]; auto.
+                 - do 2 (rewrite replace_vec_eq; auto).
+                 - do 2 (rewrite replace_vec_neq; auto).
+                 - intros. do 2 (rewrite replace_vec_neq; auto).
+            }
+            apply visible_yield_trans_schedule; auto.
+          -- (* going to i2 *)
+            exists (schedule (S n) (replace_vec v2 i2 (k' tt)) (Some i1)).
+            2: { rewrite Hequ. apply CIH. admit. admit.
+                 right. right. split; auto. split; [| split]; auto.
+                 - do 2 (rewrite replace_vec_neq; auto). symmetry; auto.
+                 - do 2 (rewrite replace_vec_eq; auto). symmetry; auto.
+                 - intros. do 2 (rewrite replace_vec_neq; auto).
+            }
+            apply visible_yield_trans_schedule; auto.
+          -- (* not going to a swapped element *)
+            exists (schedule (S n) (replace_vec v2 i2 (k' tt)) (Some i')).
+            2: { rewrite Hequ. apply CIH. admit. admit.
+                 right. left. split; auto. exists i1, i2. split; [| split; [| split]]; auto.
+                 split; [| split]; auto.
+                 - do 2 (rewrite replace_vec_eq; auto).
+                 - do 2 (rewrite replace_vec_neq; auto).
+                 - intros. do 2 (rewrite replace_vec_neq; auto).
+            }
+            apply visible_yield_trans_schedule; auto.
+      + (* the thread spawns a new thread *)
+        destruct H as (k & Hvis & Hequ).
+        destruct Hi as [
+            (? & Hv) | [
+              (? & i3 & i4 & Hneq1 & Hneq2 & Hneq3 & Hi1sb & Hi2sb & Hothers) |
+              (Hneq & Hi1sb & Hi2sb & Hothers)]].
+        * subst.
+          destruct n; try inv i2.
+          pose proof Hvis as Hvis'.
+          eapply sbisim_visible in Hvis'. 5: apply Hv. all: eauto.
+          2: { constructor. apply true. }
+          destruct Hvis' as (k' & ? & ?).
+          exists (schedule (S (S n))
+                      (cons_vec (k' true)
+                                (replace_vec v2 i2 (k' false)))
+                      (Some (Fin.FS i2))).
+          2: { rewrite Hequ. apply CIH. admit. admit.
+               left. split; auto. intros.
+               apply cons_vec_vec_relation; auto.
+               apply replace_vec_vec_relation; auto.
+          }
+          apply visible_spawn_trans_schedule; auto.
+        * subst.
+          destruct n; try inv i2.
+          pose proof Hvis as Hvis'.
+          eapply sbisim_visible in Hvis'. 5: apply Hothers; auto. all: eauto.
+          2: { constructor. apply true. }
+          destruct Hvis' as (k' & ? & ?).
+          exists (schedule (S (S n))
+                      (cons_vec (k' true)
+                                (replace_vec v2 i2 (k' false)))
+                      (Some (Fin.FS i2))).
+          2: { rewrite Hequ. apply CIH. admit. admit.
+               right. left. split; auto. exists (FS i3), (FS i4).
+               split; [| split; [| split]]; auto. admit. admit. admit.
+               split; [| split].
+               - simp cons_vec. do 2 (rewrite replace_vec_neq; auto).
+               - simp cons_vec. do 2 (rewrite replace_vec_neq; auto).
+               - intros. dependent destruction i; simp cons_vec.
+                 destruct (Fin.eq_dec i2 i).
+                 + subst. do 2 (rewrite replace_vec_eq; auto).
+                 + do 2 (rewrite replace_vec_neq; auto). apply Hothers. admit. admit.
+          }
+          apply visible_spawn_trans_schedule; auto.
+        * destruct n; try inv i2.
+          pose proof Hvis as Hvis'.
+          eapply sbisim_visible in Hvis'. 5: apply Hi1sb. all: eauto.
+          2: { constructor. apply true. }
+          destruct Hvis' as (k' & ? & ?).
+          exists (schedule (S (S n))
+                      (cons_vec (k' true)
+                                (replace_vec v2 i2 (k' false)))
+                      (Some (Fin.FS i2))).
+          2: { rewrite Hequ. apply CIH. admit. admit.
+               right. right. split. admit.
+               split; [| split].
+               - simp cons_vec. do 2 (rewrite replace_vec_eq; auto).
+               - simp cons_vec. do 2 (rewrite replace_vec_neq; auto).
+               - intros. dependent destruction i; simp cons_vec.
+                 assert (i <> i1) by admit.
+                 assert (i <> i2) by admit.
+                 do 2 (rewrite replace_vec_neq; auto).
+          }
+          apply visible_spawn_trans_schedule; auto.
+    - apply trans_schedule_obs in Ht.
+      destruct Ht as (k & i & s & ? & ? & Hvis & Hequ). inv H.
+      destruct n; try inv i.
+      pose proof Hvis as Hvis'.
+      destruct Hi as [
+          (? & Hv) | [
+            (? & i3 & i4 & Hneq1 & Hneq2 & Hneq3 & Hi1 & Hi2 & Hothers) |
+            (Hneq & Hi1 & Hi2 & Hothers)]].
+      + subst. pose proof (Hv i2).
+        eapply sbisim_visible in Hvis'. 5: apply Hv. all: eauto.
+        destruct Hvis' as (k' & ? & ?).
+        exists (schedule (S n) (replace_vec v2 i2 (k' v)) (Some i2)).
+        2: { rewrite Hequ. apply CIH; clear CIH. admit. admit.
+             left. split; auto.
+             intros. destruct (Fin.eq_dec i2 i).
+             - subst. do 2 rewrite replace_vec_eq; auto.
+             - do 2 (rewrite replace_vec_neq; auto).
+        }
+        eapply visible_stateE_trans_schedule in H0; eauto.
+      + subst. eapply sbisim_visible in Hvis'. 5: apply Hothers; auto. all: auto.
+        destruct Hvis' as (k' & ? & ?).
+        exists (schedule (S n) (replace_vec v2 i2 (k' v)) (Some i2)).
+        2: { rewrite Hequ. apply CIH; clear CIH. admit. admit.
+             right. left. split; auto.
+             exists i3, i4. split; [| split; [| split]]; auto.
+             split; [| split].
+             - do 2 (rewrite replace_vec_neq; auto).
+             - do 2 (rewrite replace_vec_neq; auto).
+             - intros. destruct (Fin.eq_dec i2 i).
+               + subst. do 2 rewrite replace_vec_eq; auto.
+               + do 2 (rewrite replace_vec_neq; auto).
+        }
+        eapply visible_stateE_trans_schedule in H; eauto.
+      + eapply sbisim_visible in Hvis'. 5: apply Hi1. all: auto.
+        destruct Hvis' as (k' & ? & ?).
+        exists (schedule (S n) (replace_vec v2 i2 (k' v)) (Some i2)).
+        2: { rewrite Hequ. apply CIH; clear CIH. admit. admit.
+             right. right. split; auto. split; [| split].
+             - do 2 rewrite replace_vec_eq; auto.
+             - do 2 (rewrite replace_vec_neq; auto).
+             - intros. do 2 (rewrite replace_vec_neq; auto).
+        }
+        eapply visible_stateE_trans_schedule in H; eauto.
+    - pose proof (trans_schedule_val_1 _ _ _ _ _ Ht). subst.
+      pose proof (trans_val_inv Ht).
+      destruct Hi as [
+          (? & Hv) | [
+            (? & i3 & i4 & Hneq1 & Hneq2 & Hneq3 & Hi1 & Hi2 & Hothers) |
+            (Hneq & Hi1 & Hi2 & Hothers)]].
+      + subst. pose proof (Hv i2). step in H0.
+        destruct H0 as [Hf _].
+        pose proof (trans_schedule_thread_val _ _ _ _ Ht) as Hv1.
+        edestruct Hf; eauto.
+        apply trans_thread_schedule_val_1 in H0. eexists; eauto. rewrite H. reflexivity.
+      + subst. specialize (Hothers i2 Hneq2 Hneq3). step in Hothers.
+        destruct Hothers as [Hf _].
+        pose proof (trans_schedule_thread_val _ _ _ _ Ht) as Hv1.
+        edestruct Hf; eauto.
+        apply trans_thread_schedule_val_1 in H0. eexists; eauto. rewrite H. reflexivity.
+      + step in Hi1. destruct Hi1 as [Hf _].
+        pose proof (trans_schedule_thread_val _ _ _ _ Ht) as Hv1.
+        edestruct Hf; eauto.
+        apply trans_thread_schedule_val_1 in H0. eexists; eauto. rewrite H. reflexivity.
+  Admitted.
+
+
+  Lemma schedule_perm_2 n (v1 v2 : vec n) i1 i2 :
+    v1 i1 ~ v2 i2 ->
+    v2 i1 ~ v1 i2 ->
+    (forall i, i <> i1 -> i <> i2 -> v1 i ~ v2 i) ->
+    schedule n v1 (Some i1) ~ schedule n v2 (Some i2).
+  Proof.
+    revert n v1 v2 i1 i2.
+    coinduction r CIH.
+    symmetric using idtac. { intros. apply H; symmetry; auto. }
+    intros n v1 v2 i1 i2 Hi1 Hi2 Hothers l t Ht. cbn in *.
+    destruct l.
+    - apply trans_schedule_thread_tau_some in Ht. 2: admit.
+      decompose [or] Ht; clear Ht.
+      + destruct H as (n' & i & Ht & ? & Hequ). subst.
+        step in Hi1. destruct Hi1 as [Hf _].
+        edestruct Hf as [? ? ?]; eauto.
+        eapply trans_thread_schedule_val_SS in H.
+        eexists. apply H. rewrite Hequ. apply CIH; cbn.
+        * admit.
+        * admit.
+        * intros. admit.
+      + destruct n; try inv i1.
+        destruct H0 as (t' & Ht & Hbound & Hequ).
+        step in Hi1. destruct Hi1 as [Hf _].
+        edestruct Hf as [? ? ?]; eauto.
+        epose proof (trans_choiceI_bound _ _ _ _ _ H).
+        apply trans_thread_schedule_tau in H.
+        eexists; eauto. rewrite Hequ. apply CIH.
+        * do 2 rewrite replace_vec_eq. auto.
+        * destruct (Fin.eq_dec i1 i2).
+          -- subst. do 2 rewrite replace_vec_eq. symmetry. auto.
+          -- do 2 (rewrite replace_vec_neq; auto).
+        * intros. do 2 (rewrite replace_vec_neq; auto).
+      + destruct H as (k & Hvis & i' & Hequ).
+        pose proof Hvis as Hvis'.
+        eapply sbisim_visible in Hvis'; eauto. 2, 3: admit.
+        destruct Hvis' as (k' & ? & ?).
+        destruct (Fin.eq_dec i' i1); [| destruct (Fin.eq_dec i' i2)]; subst.
+        { (* i1 = i' *)
+          exists (schedule n (replace_vec v2 i2 (k' tt)) (Some i2)).
+          2: {
+            rewrite Hequ. apply CIH.
+            - do 2 rewrite replace_vec_eq; auto.
+            - destruct (Fin.eq_dec i1 i2); subst.
+              + do 2 rewrite replace_vec_eq. symmetry; auto.
+              + do 2 (rewrite replace_vec_neq; auto).
+            - intros. do 2 (rewrite replace_vec_neq; auto).
+          }
+          destruct n; try inv i1.
+          apply visible_yield_trans_schedule; auto. admit.
+        }
+        { (* i1 <> i' = i2 *)
+          exists (schedule n (replace_vec v2 i2 (k' tt)) (Some i1)).
+          2: {
+            rewrite Hequ. apply CIH.
+            - do 2 (rewrite replace_vec_neq; auto). symmetry; auto.
+            - do 2 rewrite replace_vec_eq. symmetry; auto.
+            - intros. do 2 (rewrite replace_vec_neq; auto).
+          }
+          destruct n; try inv i1.
+          apply visible_yield_trans_schedule; auto. admit.
+        }
+        { (* i1 <> i' <> i2 *)
+          exists (schedule n (replace_vec v2 i2 (k' tt)) (Some i')).
+          2: {
+            rewrite Hequ. apply CIH.
+            - do 2 (rewrite replace_vec_neq; auto).
+            - do 2 (rewrite replace_vec_neq; auto). symmetry; auto.
+            - intros. destruct (Fin.eq_dec i i1); destruct (Fin.eq_dec i i2); subst.
+              + do 2 (rewrite replace_vec_eq; auto).
+              + rewrite replace_vec_eq. rewrite replace_vec_neq; auto.
+              + do 2 (rewrite replace_vec_eq; auto).
+              + do 2 (rewrite replace_vec_eq; auto).
+          }
+          destruct n; try inv i1.
+          apply visible_yield_trans_schedule; auto. admit.
+
+        }
+        destruct n; try inv i1.
+        apply visible_yield_trans_schedule; auto. admit.
+      +  destruct H as (k & Hvis & Hequ).
+         pose proof Hvis as Hvis'.
+         eapply sbisim_visible in Hvis'; eauto.
+         2: { constructor. apply true. }
+         2, 3: admit.
+         destruct Hvis' as (k' & ? & ?).
+         exists (schedule (S n)
+                     (cons_vec (k' true)
+                               (replace_vec v2 i2 (k' false)))
+                     (Some (Fin.FS i2))).
+         2: { rewrite Hequ. apply CIH.
+              - admit.
+              - admit.
+              - intros. admit.
+         }
+         destruct n; try inv i1.
+         apply visible_spawn_trans_schedule; auto. admit.
+    - apply trans_schedule_obs in Ht.
+      destruct Ht as (k & i & s & ? & ? & Hvis & Hequ). inv H.
+      destruct n; try inv i.
+      pose proof Hvis as Hvis'.
+      eapply sbisim_visible in Hvis'; eauto. 2, 3: admit.
+      destruct Hvis' as (k' & ? & ?).
+      exists (schedule (S n) (replace_vec v2 i2 (k' v)) (Some i2)).
+      2: { rewrite Hequ. apply CIH.
+           admit. admit. admit.
+      }
+      eapply visible_stateE_trans_schedule in H; eauto. admit.
+    - pose proof (trans_schedule_val_1 _ _ _ _ _ Ht). subst.
+      pose proof (trans_val_inv Ht).
+      step in Hi1. destruct Hi1 as [Hf _].
+      pose proof (trans_schedule_thread_val _ _ _ _ Ht) as Hv1.
+      edestruct Hf; eauto.
+      apply trans_thread_schedule_val_1 in H0. eexists; eauto. rewrite H. reflexivity.
+  Admitted.
+*)
 End parallel.
