examples/Yield/Lang2.v
@@ -1,0 +1,363 @@
+From Coq Require Import
+     Arith.PeanoNat
+     Lists.List
+     Strings.String
+     Morphisms
+     Setoid
+     RelationClasses.
+
+From ExtLib Require Import
+     Data.String
+     Structures.Monad
+     Structures.Traversable
+     Data.Monads.StateMonad
+     Data.List
+     Data.Map.FMapAList.
+
+(* Universe issue, TO FIX *)
+Unset Universe Checking.
+Unset Auto Template Polymorphism.
+
+From ITree Require Import
+     ITree
+     Basics.CategoryKleisli
+     Events.State
+     Events.StateFacts.
+
+From Coinduction Require Import
+	coinduction rel tactics.
+
+From CTree Require Import
+     CTree
+     Eq.
+
+From CTreeYield Require Import
+     Par2.
+
+From Equations Require Import Equations.
+
+Import ListNotations.
+Import MonadNotation.
+Local Open Scope monad_scope.
+Local Open Scope string_scope.
+
+(** Imp manipulates a countable set of variables represented as [string]s: *)
+Definition var : Set := string.
+
+(** For simplicity, the language manipulates [nat]s as values. *)
+Definition value : Type := nat.
+
+Inductive expr : Type :=
+| Var (_ : var)
+| Lit (_ : value)
+| Plus  (_ _ : expr)
+| Minus (_ _ : expr)
+| Mult  (_ _ : expr).
+
+Inductive stmt : Type :=
+| Assign (x : var) (e : expr)    (* x = e *)
+| Seq    (a b : stmt)            (* a ; b *)
+| If     (i : expr) (t e : stmt) (* if (i) then { t } else { e } *)
+| While  (t : expr) (b : stmt)   (* while (t) { b } *)
+| Spawn  (t : stmt)              (* spawn t *)
+| Skip                           (* ; *)
+.
+
+Variant ImpState : Type -> Type :=
+| GetVar (x : var) : ImpState value
+| SetVar (x : var) (v : value) : ImpState unit.
+
+Section Denote1.
+  Fixpoint denote_expr (e : expr) : ctree (spawnE +' stateE value) value :=
+    match e with
+    | Var v     => trigger (Get _)
+    | Lit n     => ret n
+    | Plus a b  => l <- denote_expr a ;; r <- denote_expr b ;; ret (l + r)
+    | Minus a b => l <- denote_expr a ;; r <- denote_expr b ;; ret (l - r)
+    | Mult a b  => l <- denote_expr a ;; r <- denote_expr b ;; ret (l * r)
+    end.
+
+  Definition while (step : ctree (spawnE +' stateE value) (unit + unit)) : ctree (spawnE +' stateE value) unit :=
+    CTree.iter (fun _ => step) tt.
+
+  Definition is_true (v : value) : bool := if (v =? 0)%nat then false else true.
+
+  Fixpoint denote_imp (s : stmt) : ctree (spawnE +' stateE value) unit :=
+    match s with
+    | Assign x e =>  v <- denote_expr e ;; trigger (Put _ v)
+    | Seq a b    =>  denote_imp a ;; denote_imp b
+    | If i t e   =>
+      v <- denote_expr i ;;
+      if is_true v then denote_imp t else denote_imp e
+
+    | While t b =>
+      while (v <- denote_expr t ;;
+	         if is_true v
+             then denote_imp b ;; ret (inl tt)
+             else ret (inr tt))
+
+    | Spawn t =>
+        b <- trigger Par2.Spawn;;
+        match b with
+        | true => denote_imp t;; ChoiceI 0 (fun _ => ret tt) (* force the thread to halt here *)
+        | false => ret tt
+        end
+    | Skip => ret tt
+
+    (* | Atomic t => translate ... (denote_imp t) *)
+    end.
+
+
+  Definition while' (step : ctree (parE value) (unit + unit)) : ctree (parE value) unit :=
+    CTree.iter (fun _ => step) tt.
+  Fixpoint denote_expr' (e : expr) : ctree (parE value) value :=
+    match e with
+    | Var v     => x <- trigger (Get _) ;; trigger Yield;; ret x
+    | Lit n     => ret n
+    | Plus a b  => l <- denote_expr' a ;; r <- denote_expr' b ;; ret (l + r)
+    | Minus a b => l <- denote_expr' a ;; r <- denote_expr' b ;; ret (l - r)
+    | Mult a b  => l <- denote_expr' a ;; r <- denote_expr' b ;; ret (l * r)
+    end.
+  Fixpoint denote_imp' (s : stmt) : ctree (parE value) unit :=
+    match s with
+    | Assign x e =>  v <- denote_expr' e ;; x <- trigger (Put _ v) ;; trigger Yield ;; ret x
+    | Seq a b    =>  denote_imp' a ;; denote_imp' b
+    | If i t e   =>
+      v <- denote_expr' i ;;
+      if is_true v then denote_imp' t else denote_imp' e
+
+    | While t b =>
+      while' (v <- denote_expr' t ;;
+	         if is_true v
+             then denote_imp' b ;; ret (inl tt)
+             else ret (inr tt))
+
+    | Spawn t =>
+        b <- trigger Par2.Spawn;;
+        match b with
+        | true => denote_imp' t;; ChoiceI 0 (fun _ => ret tt) (* force the thread to halt here *)
+        | false => ret tt
+        end
+    | Skip => ret tt
+
+    (* | Atomic t => translate ... (denote_imp t) *)
+    end.
+
+  Definition schedule_denot' (t : stmt) : thread :=
+    schedule 1 (fun _ => denote_imp' t) (Some Fin.F1).
+
+  Definition h_state : forall X, stateE value X -> ctree (parE value) X :=
+    fun _ e =>
+      match e with
+      | Get _ => x <- trigger (Get _) ;; trigger Yield ;; Ret x
+      | Put _ s' => x <- trigger (Put _ s') ;; trigger Yield ;; Ret x
+      end.
+
+  #[global] Instance MonadChoice_stateT {M S} {MM : Monad M} {AM : Utils.MonadChoice M}
+    : Utils.MonadChoice (Monads.stateT S M) :=
+    fun b n s =>
+      f <- choice b n;;
+      ret (s, f).
+
+  Definition handler : forall X, (spawnE +' stateE value) X -> ctree (parE value) X :=
+    (fun X (e : (spawnE +' stateE value) X) =>
+       match e with
+       | inl1 e' => trigger e'
+       | inr1 e' => h_state _ e'
+       end).
+
+  Definition interp_state (t : ctree (spawnE +' stateE value) unit) : thread :=
+    Interp.interp handler t.
+
+  Definition schedule_denot (t : stmt) : thread :=
+    schedule 1 (fun _ => interp_state (denote_imp t)) (Some Fin.F1).
+
+  Lemma denote_expr_bounded e :
+    choiceI_bound 1 (denote_expr' e).
+  Proof.
+    induction e; cbn; unfold trigger; auto.
+    - step. rewrite bind_vis. constructor. intros.
+      step. rewrite bind_ret_l. rewrite bind_vis. constructor. intros.
+      step. rewrite bind_ret_l. constructor.
+    - step. constructor.
+    - apply bind_choiceI_bound; auto.
+      intros. apply bind_choiceI_bound; auto.
+      intros. step. constructor.
+    - apply bind_choiceI_bound; auto.
+      intros. apply bind_choiceI_bound; auto.
+      intros. step. constructor.
+    - apply bind_choiceI_bound; auto.
+      intros. apply bind_choiceI_bound; auto.
+      intros. step. constructor.
+  Qed.
+
+  Lemma denote_stmt_bounded t :
+    choiceI_bound 1 (denote_imp' t).
+  Proof.
+    induction t; cbn.
+    - apply bind_choiceI_bound. apply denote_expr_bounded. intros.
+      step. rewrite bind_trigger. constructor. intros.
+      step. rewrite bind_trigger. constructor. intros.
+      step. constructor.
+    - apply bind_choiceI_bound; auto.
+    - apply bind_choiceI_bound. apply denote_expr_bounded.
+      intros. step. step in IHt1. step in IHt2. destruct (is_true x); auto.
+    - unfold while. apply iter_choiceI_bound; auto.
+      intros. apply bind_choiceI_bound. apply denote_expr_bounded.
+      intros. destruct (is_true x).
+      + apply bind_choiceI_bound; auto.
+        intros. step. constructor.
+      + step. constructor.
+    - apply bind_choiceI_bound.
+      + intros. step. constructor. intros. step. constructor.
+      + intros. destruct x.
+        * apply bind_choiceI_bound; auto.
+          intros. step. constructor; auto. intros. step. constructor.
+        * step. constructor.
+    - step. constructor.
+  Qed.
+
+  (* TODO: clean up proof *)
+  Lemma interp_state_bounded t :
+    choiceI_bound 1 t ->
+    choiceI_bound 1 (interp_state t).
+  Proof.
+    unfold interp_state. unfold Interp.interp. unfold iter. unfold MonadIter_ctree.
+    intros. unfold choiceI_bound. revert t H. coinduction r CIH.
+    intros. cbn. rewrite unfold_iter.
+    cbn. destruct (observe t) eqn:?; cbn. 3: destruct vis.
+    - rewrite bind_ret_l. constructor.
+    - unfold CTree.map. destruct e; destruct s; cbn.
+      + rewrite bind_trigger. rewrite bind_vis. constructor. intros.
+        rewrite bind_ret_l. step. constructor; auto.
+        intros. apply CIH. step in H. cbn in H. unfold choiceI_bound_ in H. rewrite Heqc in H.
+        inversion H. invert. apply H1.
+      + rewrite bind_trigger. do 2 rewrite bind_vis. constructor. intros.
+        rewrite bind_trigger. do 2 rewrite bind_vis. step. econstructor. intros.
+        do 2 rewrite bind_ret_l. step. constructor; auto.
+        intros. apply CIH. step in H. cbn in H. unfold choiceI_bound_ in H. rewrite Heqc in H.
+        inversion H. invert. apply H1.
+      + rewrite bind_trigger. do 2 rewrite bind_vis. constructor. intros.
+        rewrite bind_trigger. do 2 rewrite bind_vis. step. econstructor. intros.
+        do 2 rewrite bind_ret_l. step. constructor; auto.
+        intros. apply CIH. step in H. cbn in H. unfold choiceI_bound_ in H. rewrite Heqc in H.
+        inversion H. invert. apply H1.
+    - unfold choice. unfold MonadChoice_ctree. unfold CTree.choice.
+      do 2 rewrite bind_choice. constructor. intros.
+      do 2 rewrite bind_ret_l. step. constructor; auto. intros. apply CIH.
+      step in H. cbn in H. unfold choiceI_bound_ in H. rewrite Heqc in H.
+      inversion H. invert. apply H1.
+    - unfold choice. unfold MonadChoice_ctree. unfold CTree.choice.
+      do 2 rewrite bind_choice. constructor.
+      2: {
+        step in H. cbn in H. unfold choiceI_bound_ in H. rewrite Heqc in H.
+        inversion H. invert. apply H3.
+      }
+      intros.
+      do 2 rewrite bind_ret_l. step. constructor; auto. intros. apply CIH.
+      step in H. cbn in H. unfold choiceI_bound_ in H. rewrite Heqc in H.
+      inversion H. invert. apply H2.
+  Qed.
+
+  Lemma schedule_spawns t1 t2 :
+    (schedule 1 (fun _ : fin 1 => denote_imp' (Seq (Spawn t1) (Spawn t2))) (Some Fin.F1)) ≅
+    TauV (TauV (TauI (schedule 2
+                               (cons_vec
+                                  (CTree.bind (denote_imp' t2) (fun _ => ChoiceI 0 (fun _ => ret tt)))
+                                  (fun _ => CTree.bind (denote_imp' t1) (fun _ => ChoiceI 0 (fun _ => ret tt))))
+                               None))).
+  Proof.
+    rewrite rewrite_schedule. simp schedule_match.
+    cbn. CTree.fold_subst.
+    step. constructor. intros _.
+
+    rewrite rewrite_schedule. simp schedule_match. simp cons_vec.
+    unfold replace_vec. cbn.
+    step. constructor. intros _.
+
+    rewrite rewrite_schedule. simp schedule_match. simp cons_vec. cbn.
+    step. constructor. intros _.
+
+    apply equ_schedule. intro.
+    dependent destruction i.
+    - simp remove_vec. simp cons_vec. CTree.fold_subst.
+      rewrite bind_ret_l. reflexivity.
+    - dependent destruction i; [| inv i].
+      simp remove_vec. simp cons_vec.
+      unfold remove_front_vec. simp cons_vec. cbn. simp cons_vec.
+      rewrite bind_ret_l. rewrite bind_bind.
+      eapply equ_clo_bind; auto. intros; subst.
+      rewrite bind_choice. step. constructor. intros. inv i.
+  Qed.
+
+  (*
+  Lemma schedule_order (t1 t2 : ctree (parE value) unit) :
+    ChoiceV 2 (fun i' : fin 2 =>
+                 schedule 2
+                          (cons_vec t1 (fun _ => t2))
+                          (Some i')) ~
+    ChoiceV 2 (fun i' : fin 2 =>
+                 schedule 2
+                          (cons_vec t2 (fun _ => t1))
+                          (Some i')).
+  Proof.
+    apply sb_choiceV; intros i.
+    - dependent destruction i.
+      + exists (Fin.FS Fin.F1). rewrite schedule_perm_2; auto.
+        intros. exfalso. dependent destruction i; auto.
+        dependent destruction i; auto. inv i.
+      + exists (Fin.F1). rewrite schedule_perm_2; auto.
+        intros. exfalso. dependent destruction i0; auto.
+        dependent destruction i; try inv i.
+        dependent destruction i0; try inv i0. auto.
+    - dependent destruction i.
+      + exists (Fin.FS Fin.F1). rewrite schedule_perm_2; auto.
+        intros. exfalso. dependent destruction i; auto.
+        dependent destruction i; auto. inv i.
+      + exists (Fin.F1). rewrite schedule_perm_2; auto.
+        intros. exfalso. dependent destruction i0; auto.
+        dependent destruction i; try inv i.
+        dependent destruction i0; try inv i0. auto.
+  Qed.
+
+  (*   (* permutation lemma would solve immediately *) *)
+  (*   revert t1 t2. *)
+  (*   coinduction r CIH. intros. *)
+  (*   apply step_sb_choiceV; intros i. *)
+  (*   - dependent destruction i. *)
+  (*     + exists (Fin.FS Fin.F1). *)
+  (*       do 2 rewrite rewrite_schedule. simp schedule_match. simp cons_vec. *)
+  (*       destruct (observe t1); cbn. *)
+  (*       * step. apply step_sb_tauI. rewrite remove_vec_1, remove_vec_2. reflexivity. *)
+  (*       * destruct e; [destruct y | destruct s; [destruct s |]]. *)
+  (*         -- setoid_rewrite <- (bind_ret_l tt (fun _ => schedule _ _ _)). *)
+  (*            do 2 rewrite <- bind_tauI. *)
+  (*            apply st_clo_bind; auto. (* TODO: put into separate lemma *) *)
+  (*            intros. *)
+  (*            do 2 rewrite rewrite_schedule. simp schedule_match. *)
+  (*            rewrite replace_vec_1, replace_vec_2. *)
+  (*            apply CIH. *)
+  (*         -- rewrite replace_vec_1, replace_vec_2. *)
+  (*            setoid_rewrite <- (bind_ret_l tt (fun _ => schedule _ _ _)). *)
+  (*            do 2 rewrite <- bind_tauV. *)
+  (*            apply st_clo_bind; auto. *)
+  (*            intros. admit. (* permutation lemma? *) *)
+  (*         -- do 2 rewrite <- bind_trigger. *)
+  (*            apply st_clo_bind; auto. *)
+  (*            intros. *)
+  (*            rewrite replace_vec_1, replace_vec_2. *)
+  (*            admit. (* also permutation lemma *) *)
+  (* Admitted. *)
+
+  Lemma commut_spawns t1 t2 :
+    schedule_denot' (Seq (Spawn t1) (Spawn t2)) ~
+    schedule_denot' (Seq (Spawn t2) (Spawn t1)).
+  Proof.
+    unfold schedule_denot'.
+    do 2 rewrite schedule_spawns.
+    apply sb_tauV. apply sb_tauV. apply sb_tauI_lr.
+    do 2 rewrite rewrite_schedule. simp schedule_match.
+    apply schedule_order.
+  Qed.
+*)
+End Denote1.
